src3.0/Transforms/alive_alloca.v
@@ -11,6 +11,7 @@ Require Import primitives.
 Require Import palloca_props.
 Require Import memory_props.
 Require Import trans_tactic.
+Require Import alive_mop.
 
 Import Promotability.
 
@@ -25,11 +26,42 @@ exists cs1, exists cs3,
   cs2 ++
   cs3.
 
+Lemma alive_alloca__alive_mop: forall (cs2:cmds) (b:block) (pinfo:PhiInfo)
+  (H: alive_alloca cs2 b pinfo),
+  alive_mop (value_const (const_undef (PI_typ pinfo))) 
+    (insn_alloca (PI_id pinfo) (PI_typ pinfo) (PI_num pinfo) (PI_align pinfo)) 
+    cs2 b pinfo.
+Proof.
+  intros. destruct b as [? []].
+  destruct H as [J1 [J2 [? [? ?]]]]; subst. 
+  unfold alive_mop. repeat (split; eauto). 
+Qed.
+
 Record AllocaInfo (pinfo: PhiInfo) := mkAllocaInfo {
   AI_tail : cmds;
   AI_block : block;
   AI_alive : alive_alloca AI_tail AI_block pinfo
 }.
+
+Definition alinfo__eq__minfo pinfo ainfo minfo: Prop :=
+M_value pinfo minfo = value_const (const_undef (PI_typ pinfo)) /\
+M_c pinfo minfo = 
+      insn_alloca (PI_id pinfo) (PI_typ pinfo) (PI_num pinfo) (PI_align pinfo) /\
+M_tail pinfo minfo = AI_tail pinfo ainfo /\
+M_block pinfo minfo = AI_block pinfo ainfo.
+
+Lemma alinfo__minfo: forall pinfo (ainfo: AllocaInfo pinfo), 
+  { minfo: MopInfo pinfo | alinfo__eq__minfo pinfo ainfo minfo }.
+Proof.  
+  intros.
+  destruct ainfo. 
+  exists (mkMopInfo pinfo
+    (value_const (const_undef (PI_typ pinfo)))
+    (insn_alloca (PI_id pinfo) (PI_typ pinfo) (PI_num pinfo) (PI_align pinfo))
+    AI_tail0 AI_block0 
+    (alive_alloca__alive_mop AI_tail0 AI_block0 pinfo AI_alive0)).
+  split; auto.
+Qed.
 
 Definition wf_defs (pinfo:PhiInfo) (alinfo: AllocaInfo pinfo) TD M gl (lc:DGVMap)
   : Prop :=
@@ -38,6 +70,15 @@ forall gvsa gvsv
   (Hlkpv: Opsem.getOperandValue TD (value_const (const_undef (PI_typ pinfo))) lc
      gl = Some gvsv),
   mload TD M gvsa (PI_typ pinfo) (PI_align pinfo) = Some gvsv.
+
+Lemma alinfo__wf_defs__minfo: forall (pinfo:PhiInfo) (alinfo: AllocaInfo pinfo) 
+  TD M gl (lc:DGVMap) minfo (Heq: alinfo__eq__minfo pinfo alinfo minfo),
+  wf_defs pinfo alinfo TD M gl lc <-> alive_mop.wf_defs pinfo minfo TD M gl lc.
+Proof.
+  intros. destruct Heq as [J1 [J2 [J3 J4]]].
+  unfold wf_defs, alive_mop.wf_defs.
+  rewrite J1. tauto.
+Qed.
 
 Definition follow_alive_alloca (pinfo:PhiInfo) (alinfo: AllocaInfo pinfo)
   (cs:cmds) : Prop :=
@@ -51,44 +92,15 @@ forall cs1 cs3,
   (exists csa, exists csb,
     cs = csb ++ cs3 /\ AI_tail pinfo alinfo = csa ++ csb).
 
-Lemma follow_alive_alloca_cons: forall pinfo alinfo c cs l0 ps0 cs0 tmn0
-  (Huniq:uniqFdef (PI_f pinfo)) (Hneq: getCmdLoc c <> PI_id pinfo),
-  (l0, stmts_intro ps0 (cs0++c::cs) tmn0) = AI_block pinfo alinfo ->
-  store_in_cmd (PI_id pinfo) c = false ->
-  follow_alive_alloca pinfo alinfo cs ->
-  follow_alive_alloca pinfo alinfo (c::cs).
+Lemma alinfo__follow_alive__minfo: forall (pinfo:PhiInfo) 
+  (alinfo: AllocaInfo pinfo) cs minfo 
+  (Heq: alinfo__eq__minfo pinfo alinfo minfo),
+  follow_alive_alloca pinfo alinfo cs <-> 
+    alive_mop.follow_alive_mop pinfo minfo cs.
 Proof.
-  unfold follow_alive_alloca.
-  intros.
-  destruct alinfo. simpl in *.
-  unfold alive_alloca in AI_alive0.
-  destruct AI_block0 as [? []].
-  destruct AI_alive0 as [J1 [J2 [cs1 [cs3 J3]]]]; subst.
-  intros.
-  assert (cs1 = cs2 /\ cs3 = cs4) as J.
-    eapply uniqFdef_cmds_split_middle in H2; eauto.
-    destruct H2 as [G1 G2].
-    split; auto.
-      apply app_inv_head in G2; auto.
-
-  destruct J as [EQ1 EQ2]; subst. clear H2.
-  edestruct H1 as [csa [csb [EQ1 EQ2]]]; eauto. clear H1.
-  subst. inv H.
-  anti_simpl_env.
-  destruct csa.
-    anti_simpl_env.
-    contradict Hneq; auto.
-
-    assert (exists csa', exists c2, [c0] ++ csa = csa' ++ [c2]) as EQ.
-      apply head_tail_commut.
-    destruct EQ as [csa' [c2 EQ]].
-    simpl_env in H4.
-    rewrite EQ in H4.
-    anti_simpl_env.
-    exists csa'. exists (c2::csb). simpl_env.
-    rewrite_env (([c0] ++ csa) ++ csb).
-    rewrite EQ. simpl_env.
-    split; auto.
+  intros. destruct Heq as [J1 [J2 [J3 J4]]].
+  unfold follow_alive_alloca, alive_mop.follow_alive_mop.
+  rewrite J4. rewrite J2. rewrite J3. tauto.
 Qed.
 
 Definition wf_ExecutionContext (pinfo:PhiInfo) (alinfo: AllocaInfo pinfo) TD M gl
@@ -97,6 +109,23 @@ Opsem.CurFunction ec = PI_f pinfo ->
 Opsem.CurBB ec = AI_block pinfo alinfo ->
 follow_alive_alloca pinfo alinfo (Opsem.CurCmds ec) ->
 wf_defs pinfo alinfo TD M gl (Opsem.Locals ec).
+
+Lemma alinfo__wf_EC__minfo: forall (pinfo:PhiInfo) (alinfo: AllocaInfo pinfo) 
+  TD M gl ec minfo (Heq: alinfo__eq__minfo pinfo alinfo minfo),
+  wf_ExecutionContext pinfo alinfo TD M gl ec <-> 
+    alive_mop.wf_ExecutionContext pinfo minfo TD M gl ec.
+Proof.
+  intros.
+  unfold wf_ExecutionContext, alive_mop.wf_ExecutionContext.
+  assert (J:=Heq).
+  apply alinfo__follow_alive__minfo with (cs:=Opsem.CurCmds ec) in J.
+  assert (J':=Heq).
+  apply alinfo__wf_defs__minfo with (lc:=Opsem.Locals ec)(TD:=TD)(M:=M)
+    (gl:=gl) in J'.
+  destruct Heq as [J1 [J2 [J3 J4]]].
+  rewrite J4.
+  tauto.
+Qed.
 
 Fixpoint wf_ECStack (pinfo:PhiInfo) (alinfo: AllocaInfo pinfo) TD M gl
   (ecs:Opsem.ECStack) : Prop :=
@@ -107,806 +136,32 @@ match ecs with
     wf_ECStack pinfo alinfo TD M gl ecs'
 end.
 
+Lemma alinfo__wf_ECs__minfo: forall (pinfo:PhiInfo) (alinfo: AllocaInfo pinfo) 
+  TD M gl minfo (Heq: alinfo__eq__minfo pinfo alinfo minfo) ecs,
+  wf_ECStack pinfo alinfo TD M gl ecs <-> 
+    alive_mop.wf_ECStack pinfo minfo TD M gl ecs.
+Proof.
+  induction ecs.
+    tauto.
+   
+    assert (J:=Heq).
+    apply alinfo__wf_EC__minfo with (ec:=a)(TD:=TD)(M:=M)(gl:=gl) in J.
+    simpl. tauto.
+Qed.
+
 Definition wf_State (pinfo:PhiInfo) (alinfo: AllocaInfo pinfo)
   (cfg:OpsemAux.Config) (S:Opsem.State) : Prop :=
 wf_ECStack pinfo alinfo (OpsemAux.CurTargetData cfg) (Opsem.Mem S)
   (OpsemAux.Globals cfg) (Opsem.ECS S).
 
-(* its proof is same to alive_store.v *)
-Lemma free_allocas_preserves_wf_defs: forall pinfo TD Mem lc' als0 als Mem'
-  gl alinfo maxb,
-  Promotability.wf_defs maxb pinfo TD Mem lc' als0 ->
-  wf_defs pinfo alinfo TD Mem gl lc' ->
-  NoDup (als ++ als0) ->
-  free_allocas TD Mem als = ret Mem' ->
-  wf_defs pinfo alinfo TD Mem' gl lc'.
-Proof.
-  intros. unfold wf_defs in *. intros.
-  assert (Hlkpa':=Hlkpa).
-  eapply H0 in Hlkpa; eauto. clear H0.
-  eapply H in Hlkpa'; eauto.
-  destruct Hlkpa' as [J1 J2].
-  destruct J1 as [_ [[mb [J1 [J3 J4]]] _]]; subst.
-  eapply alist.NoDup_disjoint in H1; eauto.
-  eapply free_allocas_preserves_mload; eauto.
-Qed.
-
-Lemma wf_defs_updateAddAL: forall pinfo alinfo TD M lc' i1 gv1 gl
-  (HwfDef: wf_defs pinfo alinfo TD M gl lc')
-  (Hneq: i1 <> PI_id pinfo),
-  wf_defs pinfo alinfo TD M gl (updateAddAL _ lc' i1 gv1).
-Proof.
-  intros. unfold wf_defs in *. intros.
-  rewrite <- lookupAL_updateAddAL_neq in Hlkpa; auto.
-Qed.
-
-(* its proof is same to alive_store.v *)
-Lemma free_allocas_preserves_wf_ECStack: forall maxb pinfo alinfo td als gl ECs
-  Mem Mem'
-  (HwfECs : Promotability.wf_ECStack maxb pinfo td Mem ECs)
-  (Hwfpi: WF_PhiInfo pinfo)
-  (Hndup: NoDup (als ++ (flat_map
-                  (fun ec : Opsem.ExecutionContext =>
-                   let '{| Opsem.Allocas := als |} := ec in als)
-                   ECs)))
-  (Hwf: wf_ECStack pinfo alinfo td Mem gl ECs)
-  (Hfrees: free_allocas td Mem als = ret Mem'),
-  wf_ECStack pinfo alinfo td Mem' gl ECs.
-Proof.
-  induction ECs as [|[]]; simpl; intros; auto.
-    destruct Hwf as [J1 J2].
-    assert (Hndup' := Hndup).
-    apply NoDup_strenthening in Hndup.
-    destruct HwfECs as [[Hwfdefs _] [HwfECs _]].
-    split; eauto.
-      intros G1 G2 G3. simpl in G1, G2, G3. subst. simpl.
-      apply J1 in G3; auto. simpl in G3.
-      destruct (fdef_dec (PI_f pinfo) (PI_f pinfo)); try congruence.
-      rewrite_env ((als ++ Allocas) ++
-        flat_map
-          (fun ec : Opsem.ExecutionContext =>
-           let '{| Opsem.Allocas := als |} := ec in als) ECs) in Hndup'.
-      apply NoDup_split in Hndup'. destruct Hndup'.
-      eapply free_allocas_preserves_wf_defs in G3; eauto.
-Qed.
-
-Lemma follow_alive_alloca_at_beginning_false: forall (pinfo : PhiInfo)
-  (alinfo : AllocaInfo pinfo) (l' : l) (ps' : phinodes) (cs' : cmds)
-  (tmn' : terminator)
-  (J2 : (l', stmts_intro ps' cs' tmn') = AI_block pinfo alinfo)
-  (J3 : follow_alive_alloca pinfo alinfo cs'),
-  False.
+Lemma alinfo__wf_State__minfo: forall (pinfo:PhiInfo) (alinfo: AllocaInfo pinfo) 
+  minfo (Heq: alinfo__eq__minfo pinfo alinfo minfo) cfg S,
+  wf_State pinfo alinfo cfg S <-> 
+    alive_mop.wf_State pinfo minfo cfg S.
 Proof.
   intros.
-  unfold follow_alive_alloca in J3.
-  rewrite <- J2 in J3.
-  destruct alinfo. simpl in *.
-  rewrite <- J2 in AI_alive0.
-  destruct AI_alive0 as [_ [_ [cs1 [cs3 J]]]].
-  assert (J':=J).
-  apply J3 in J.
-  destruct J as [csa [csb [EQ1 EQ2]]]; subst.
-  anti_simpl_env.
+  apply alinfo__wf_ECs__minfo; auto.
 Qed.
-
-Ltac preservation_sBranch :=
-match goal with
-| HwfS1 : wf_State _ _ _ _ |- _ =>
-  destruct HwfS1 as [_ HwfECs];
-  simpl in HwfECs;
-  fold wf_ECStack in HwfECs;
-  split; try solve [
-    auto |
-    intros J1 J2 J3; simpl in *; subst;
-    eapply follow_alive_alloca_at_beginning_false in J3; eauto;
-    inv J3]
-end.
-
-Lemma preservation_return : forall maxb pinfo alinfo (HwfPI : WF_PhiInfo pinfo)
-  F B rid RetTy Result lc F' B' c' cs' tmn' lc' EC Mem als als' cfg
-  EC1 EC2
-  (EQ1:EC1 = {| Opsem.CurFunction := F;
-                Opsem.CurBB := B;
-                Opsem.CurCmds := nil;
-                Opsem.Terminator := insn_return rid RetTy Result;
-                Opsem.Locals := lc;
-                Opsem.Allocas := als |})
-  (EQ2:EC2 = {| Opsem.CurFunction := F';
-                Opsem.CurBB := B';
-                Opsem.CurCmds := c' :: cs';
-                Opsem.Terminator := tmn';
-                Opsem.Locals := lc';
-                Opsem.Allocas := als' |})
-  (Hwfcfg : OpsemPP.wf_Config cfg)
-  (Hwfpp : OpsemPP.wf_State cfg
-           {| Opsem.ECS := EC1 :: EC2 :: EC;
-              Opsem.Mem := Mem |})
-  (Hnoalias : Promotability.wf_State maxb pinfo cfg
-           {| Opsem.ECS := EC1 :: EC2 :: EC;
-              Opsem.Mem := Mem |})
-  Mem' lc'' (H : Instruction.isCallInst c' = true)
-  (H0 : free_allocas (OpsemAux.CurTargetData cfg) Mem als = ret Mem')
-  (H1 : Opsem.returnUpdateLocals
-          (OpsemAux.CurTargetData cfg) c'
-            Result lc lc' (OpsemAux.Globals cfg) = ret lc'')
-  (HwfS1 : wf_State pinfo alinfo cfg
-            {| Opsem.ECS := EC1 :: EC2 :: EC;
-               Opsem.Mem := Mem |}),
-  wf_State pinfo alinfo cfg
-     {| Opsem.ECS :=
-             {| Opsem.CurFunction := F';
-                Opsem.CurBB := B';
-                Opsem.CurCmds := cs';
-                Opsem.Terminator := tmn';
-                Opsem.Locals := lc'';
-                Opsem.Allocas := als' |} :: EC;
-        Opsem.Mem := Mem' |}.
-Proof.
-  intros. subst. destruct cfg as [S [los nts] Ps gl fs].
-
-  destruct Hwfcfg as [_ [_ [HwfSystem HmInS]]].
-  destruct Hwfpp as 
-    [_ [_ 
-     [
-       [
-         [_ [HBinF1 [HFinPs1 [_ [_ [l2 [ps2 [cs2' Heq2]]]]]]]]
-         _
-       ]
-       _
-     ]
-    ]]; subst.
-
-  destruct HwfS1 as [Hinscope1 [Hinscope2 HwfECs]]. simpl.
-  simpl in Hinscope1, Hinscope2, HwfECs.
-  fold wf_ECStack in HwfECs.
-
-  destruct Hnoalias as
-    [
-      [_ [[[Hinscope2' _] [HwfECs' _]] _]]
-      [[Hdisjals _] HwfM]
-    ]. simpl in Hdisjals.
-  fold Promotability.wf_ECStack in HwfECs'.
-
-  split.
-    SSCase "wf_EC".
-    intros J1 J2 J3. simpl in J1, J2, J3. simpl. subst.
-    remember (getCmdID c') as R.
-    destruct_cmd c'; try solve [inversion H].
-    unfold wf_ExecutionContext in *. simpl in Hinscope1, Hinscope2.
-    assert (J2':=J2).
-    assert (uniqFdef (PI_f pinfo)) as Huniq. eauto using wf_system__uniqFdef.
-    assert (getCmdLoc (insn_call i0 n c t0 v0 v p) <> PI_id pinfo) as Hneq.
-      apply WF_PhiInfo_spec10 in HBinF1; auto.
-    apply follow_alive_alloca_cons in J2; auto.
-    assert (J2'':=J2).
-    apply Hinscope2 in J2; auto.
-    assert (NoDup (als ++ als')) as Hnodup.
-      rewrite_env
-        ((als ++ als') ++
-          flat_map
-            (fun ec : Opsem.ExecutionContext =>
-             let '{| Opsem.Allocas := als |} := ec in als) EC) in Hdisjals.
-      apply NoDup_split in Hdisjals.
-      destruct Hdisjals; auto.
-    destruct (fdef_dec (PI_f pinfo) (PI_f pinfo)); try congruence.
-    eapply free_allocas_preserves_wf_defs in J2; eauto. clear Hnodup.
-      unfold Opsem.returnUpdateLocals in H1. simpl in H1.
-      remember (Opsem.getOperandValue (los,nts) Result lc gl) as R1.
-      destruct R1; try solve [inv H1].
-      destruct R.
-      SSSSSCase "c' defines a variable".
-        destruct n; inv HeqR.
-        remember (lift_op1 DGVs (fit_gv (los, nts) t0) g t0) as R2.
-        destruct R2; inv H1.
-        apply wf_defs_updateAddAL; auto.
-
-      SSSSSCase "c' defines nothing".
-        destruct n; inv HeqR. inv H1. auto.
-
-    SSCase "wf_ECs".
-      simpl.
-      eapply free_allocas_preserves_wf_ECStack; eauto.
-      apply NoDup_strenthening in Hdisjals; auto.
-Qed.
-
-Lemma preservation_return_void : forall maxb pinfo alinfo
-  (HwfPI : WF_PhiInfo pinfo)
-  F B rid lc F' B' c' cs' tmn' lc' EC Mem als als' cfg EC1 EC2
-  (EQ1:EC1 = {| Opsem.CurFunction := F;
-                Opsem.CurBB := B;
-                Opsem.CurCmds := nil;
-                Opsem.Terminator := insn_return_void rid;
-                Opsem.Locals := lc;
-                Opsem.Allocas := als |})
-  (EQ2:EC2 = {| Opsem.CurFunction := F';
-                Opsem.CurBB := B';
-                Opsem.CurCmds := c' :: cs';
-                Opsem.Terminator := tmn';
-                Opsem.Locals := lc';
-                Opsem.Allocas := als' |})
-  (Hwfcfg : OpsemPP.wf_Config cfg)
-  (Hwfpp : OpsemPP.wf_State cfg
-           {| Opsem.ECS := EC1 :: EC2 :: EC;
-              Opsem.Mem := Mem |})
-  (Hnoalias : Promotability.wf_State maxb pinfo cfg
-           {| Opsem.ECS := EC1 :: EC2 :: EC;
-              Opsem.Mem := Mem |})
-  Mem' (H : Instruction.isCallInst c' = true)
-  (H0 : free_allocas (OpsemAux.CurTargetData cfg) Mem als = ret Mem')
-  (HwfS1 : wf_State pinfo alinfo cfg
-            {| Opsem.ECS := EC1 :: EC2 :: EC;
-               Opsem.Mem := Mem |}),
-  wf_State pinfo alinfo cfg
-     {| Opsem.ECS :=
-             {| Opsem.CurFunction := F';
-                Opsem.CurBB := B';
-                Opsem.CurCmds := cs';
-                Opsem.Terminator := tmn';
-                Opsem.Locals := lc';
-                Opsem.Allocas := als' |} :: EC;
-        Opsem.Mem := Mem' |}.
-Proof.
-  intros. subst. destruct cfg as [S [los nts] Ps gl fs].
-  destruct Hwfcfg as [_ [_ [HwfSystem HmInS]]].
-  destruct Hwfpp as 
-    [_ [_ 
-     [
-       [
-         [_ [HBinF1 [HFinPs1 [_ [_ [l2 [ps2 [cs2' Heq2]]]]]]]]
-         _
-       ]
-       _
-     ]
-    ]]; subst.
-
-  destruct HwfS1 as [Hinscope1 [Hinscope2 HwfECs]]. simpl.
-  simpl in Hinscope1, Hinscope2, HwfECs.
-  fold wf_ECStack in HwfECs.
-
-  destruct Hnoalias as
-    [
-      [_ [[[Hinscope2' _] [HwfECs' _]] _]]
-      [[Hdisjals _] HwfM]
-    ]. simpl in Hdisjals.
-  fold Promotability.wf_ECStack in HwfECs'.
-
-  split.
-    SSCase "wf_EC".
-    intros J1 J2 J3. simpl in J1, J2, J3. simpl. subst.
-    remember (getCmdID c') as R.
-    destruct_cmd c'; try solve [inversion H].
-    unfold wf_ExecutionContext in *. simpl in Hinscope1, Hinscope2.
-    assert (J2':=J2).
-    assert (Huniq: uniqFdef (PI_f pinfo)) by eauto using wf_system__uniqFdef.
-    assert (getCmdLoc (insn_call i0 n c t0 v0 v p) <> PI_id pinfo) as Hneq.
-      apply WF_PhiInfo_spec10 in HBinF1; auto.
-    apply follow_alive_alloca_cons in J2; auto.
-    apply Hinscope2 in J2; auto.
-    assert (NoDup (als ++ als')) as Hnodup.
-      rewrite_env
-        ((als ++ als') ++
-          flat_map
-            (fun ec : Opsem.ExecutionContext =>
-             let '{| Opsem.Allocas := als |} := ec in als) EC) in Hdisjals.
-      apply NoDup_split in Hdisjals.
-      destruct Hdisjals; auto.
-    destruct (fdef_dec (PI_f pinfo) (PI_f pinfo)); try congruence.
-    eapply free_allocas_preserves_wf_defs in J2; eauto.
-
-    SSCase "wf_ECs".
-      simpl.
-      eapply free_allocas_preserves_wf_ECStack; eauto.
-      apply NoDup_strenthening in Hdisjals; auto.
-Qed.
-
-Lemma malloc_preserves_wf_EC_at_head : forall pinfo los nts Ps M
-  (Hwfpi:WF_PhiInfo pinfo) s als' (Hwfpi: WF_PhiInfo pinfo)
-  M' gl als lc t mb id0 align0 F gn tsz l1 ps1 cs1' cs tmn
-  (HwfF: wf_fdef s (module_intro los nts Ps) F) (HuniqF: uniqFdef F)
-  (Hsz: getTypeAllocSize (los, nts) t = ret tsz)
-  (Hal: malloc (los,nts) M tsz gn align0 = ret (M', mb)) alinfo c
-  (HBinF: blockInFdefB
-             (l1, stmts_intro ps1 (cs1' ++ c :: cs)
-                tmn) F = true)
-  (Hid : getCmdID c = Some id0)
-  (Hnst : store_in_cmd (PI_id pinfo) c = false)
-  (Hsort : match c with
-           | insn_malloc _ t0 _ _ | insn_alloca _ t0 _ _ => t = t0
-           | _ => False
-           end)
-  (Hinscope : wf_ExecutionContext pinfo alinfo (los,nts) M gl
-               {|
-               Opsem.CurFunction := F;
-               Opsem.CurBB := (l1, stmts_intro ps1
-                                (cs1' ++ c :: cs)
-                                tmn);
-               Opsem.CurCmds := c :: cs;
-               Opsem.Terminator := tmn;
-               Opsem.Locals := lc;
-               Opsem.Allocas := als |}),
-  wf_ExecutionContext pinfo alinfo (los,nts) M' gl
-    {|
-    Opsem.CurFunction := F;
-    Opsem.CurBB := (l1, stmts_intro ps1
-                      (cs1' ++ c :: cs) tmn);
-    Opsem.CurCmds := cs;
-    Opsem.Terminator := tmn;
-    Opsem.Locals := updateAddAL (GVsT DGVs) lc id0
-                       ($ blk2GV (los,nts) mb # typ_pointer t $);
-    Opsem.Allocas := als' |}.
-Proof.
-  intros.
-  intros J1 J2 J3. simpl in J1, J2, J3. simpl. subst.
-  assert (J2':=J2).
-  destruct (id_dec id0 (PI_id pinfo)); subst.
-  Case "id0 = PI_id pinfo".
-        destruct_cmd c; tinv Hsort.
-        SCase "c = malloc".
-          apply getCmdLoc_getCmdID in Hid; subst.
-          eapply WF_PhiInfo_spec10 in HBinF; eauto.
-            clear - Hid HBinF.
-            contradict Hid; auto.
-
-        SCase "c = alloca".
-          inv Hid.
-          assert (wf_typ s (los,nts) t0) as Hwft.
-            eapply wf_fdef__wf_cmd in HBinF; eauto using in_middle.
-            inv HBinF. auto.
-          clear - J2' J3 HwfF Hal Hsz Hwft HuniqF Hwfpi. 
-          unfold follow_alive_alloca in J3.
-          rewrite <- J2' in J3.
-          destruct alinfo. simpl in *. subst.
-          destruct AI_alive0 as [J1 [J5 [cs1 [cs2 J4]]]].
-          assert (J4':=J4).
-          apply J3 in J4'. clear J3.
-          destruct J4' as [csa [csb [EQ1 EQ2]]]; subst.
-                    unfold wf_defs. intros.
-          rewrite lookupAL_updateAddAL_eq in Hlkpa. inv Hlkpa.
-          simpl in Hlkpv.
-          anti_simpl_env.
-          assert (t0 = PI_typ pinfo) as Heqt.
-            simpl in J1.
-            apply WF_PhiInfo_spec1' in J1; auto. inv J1. auto.
-          subst.
-          eapply malloc_mload_undef; eauto.
-
-  Case "id0 <> PI_id pinfo".
-    apply getCmdLoc_getCmdID in Hid. subst.
-    apply follow_alive_alloca_cons in J2; auto.
-    apply Hinscope in J2; auto. simpl in J2.
-    destruct (fdef_dec (PI_f pinfo) (PI_f pinfo)); try congruence.
-    apply wf_defs_updateAddAL with (i1:=getCmdLoc c)
-      (gv1:=($ blk2GV (los,nts) mb # typ_pointer t $)) in J2; auto.
-      intros gvsa gvsv Hlkpa Hlkpv.
-      eapply J2 in Hlkpv; eauto.
-      eapply malloc_preserves_mload; eauto.
-Qed.
-
-(* its proof is same to alive_store.v *)
-Lemma malloc_preserves_wf_EC_in_tail : forall pinfo td M
-  EC M' gl mb align0 gn tsz
-  (Hal: malloc td M tsz gn align0 = ret (M', mb)) alinfo
-  (Hinscope : wf_ExecutionContext pinfo alinfo td M gl EC),
-  wf_ExecutionContext pinfo alinfo td M' gl EC.
-Proof.
-  intros.
-  intros J1 J2 J3.
-  apply Hinscope in J3; auto.
-  intros gvsa gvsv Hlkpa Hlkpv.
-  eapply J3 in Hlkpv; eauto.
-  eapply malloc_preserves_mload; eauto.
-Qed.
-
-(* its proof is same to alive_store.v *)
-Lemma malloc_preserves_wf_ECStack_in_tail : forall pinfo alinfo TD M tsz gn
-  align0 (Hwfpi: WF_PhiInfo pinfo) M' mb gl
-  (Hmlc: malloc TD M tsz gn align0 = ret (M', mb)) ECs
-  (Hwf: wf_ECStack pinfo alinfo TD M gl ECs),
-  wf_ECStack pinfo alinfo TD M' gl ECs.
-Proof.
-  induction ECs; simpl; intros; auto.
-    destruct Hwf as [J1 J2].
-    split; auto.
-      eapply malloc_preserves_wf_EC_in_tail; eauto.
-Qed.
-
-(* same to alive_store.v *)
-Ltac destruct_ctx_other :=
-match goal with
-| Hwfcfg : OpsemPP.wf_Config _, Hwfpp : OpsemPP.wf_State _ _,
-  HwfS1 : wf_State _ _ _ _,
-  Hnoalias : Promotability.wf_State _ _ _ _ |- _ =>
-  destruct Hwfcfg as [_ [_ [HwfSystem HmInS]]];
-  destruct Hwfpp as 
-    [Hnonempty [
-     [Hreach1 [HBinF1 [HFinPs1 [_ [_ [l1 [ps1 [cs1' Heq1]]]]]]]]
-     [HwfEC0 HwfCall]
-    ]]; subst;
-  fold (@OpsemPP.wf_ECStack DGVs) in HwfEC0;
-  destruct HwfS1 as [Hinscope HwfECs]; simpl;
-  simpl in Hinscope, HwfECs;
-  fold wf_ECStack in HwfECs;
-  destruct Hnoalias as
-    [
-      [[Hinscope' _] [HwfECs' HwfHT]]
-      [[Hdisjals _] HwfM]
-    ]; simpl in Hdisjals;
-  fold Promotability.wf_ECStack in HwfECs'
-end.
-
-(* its proof is same to alive_store.v *)
-Lemma free_preserves_wf_EC_in_tail : forall pinfo los nts M EC M' mptr0
-  maxb gl (Hwfg: wf_globals maxb gl) Ps S F t
-  (Hfree: free (los,nts) M mptr0 = ret M') stinfo mptrs v lc
-  (Hwft: wf_value S (module_intro los nts Ps) F v t)
-  (H : Opsem.getOperandValue (los,nts) v lc gl = ret mptrs)
-  (H0 : mptr0 @ mptrs)
-  (Hinscope : wf_ExecutionContext pinfo stinfo (los,nts) M gl EC)
-  (Hht : wf_ECStack_head_in_tail maxb pinfo (los,nts) M lc EC),
-  wf_ExecutionContext pinfo stinfo (los,nts) M' gl EC.
-Proof.
-  intros.
-  intros J1 J2 J3.
-  apply Hinscope in J3; auto.
-  intros gvsa gvsv Hlkpa Hlkpv.
-  eapply J3 in Hlkpv; eauto.
-  eapply free_preserves_mload; eauto.
-    eapply operand__no_alias_with__tail; eauto.
-Qed.
-
-(* its proof is same to alive_store.v *)
-Lemma free_preserves_wf_ECStack_in_tail : forall maxb pinfo stinfo los nts M
-  (Hwfpi: WF_PhiInfo pinfo) M' gl mptr0 (Hwfg: wf_globals maxb gl)
-  (Hfree: free (los,nts) M mptr0 = ret M') lc mptrs v t S Ps F
-  (Hwft: wf_value S (module_intro los nts Ps) F v t)
-  (H : Opsem.getOperandValue (los,nts) v lc gl = ret mptrs)
-  (H0 : mptr0 @ mptrs) ECs
-  (Hhts: wf_ECStack_head_tail maxb pinfo (los,nts) M lc ECs)
-  (Hwf: wf_ECStack pinfo stinfo (los,nts) M gl ECs),
-  wf_ECStack pinfo stinfo (los,nts) M' gl ECs.
-Proof.
-  induction ECs; simpl; intros; auto.
-    destruct Hwf as [J1 J2].
-    apply wf_ECStack_head_tail_cons__inv in Hhts.
-    destruct Hhts as [J3 J4].
-    split; auto.
-      eapply free_preserves_wf_EC_in_tail; eauto.
-Qed.
-
-Lemma preservation_pure_cmd_updated_case : forall (F : fdef)(B : block)
-  (lc : DGVMap)(gv3 : GVsT DGVs) (cs : list cmd) (tmn : terminator) id0 c0 Mem0
-  als ECs pinfo alinfo
-  (HwfPI : WF_PhiInfo pinfo) (Hid : getCmdID c0 = Some id0) cfg maxb EC
-  (Heq: EC = {| Opsem.CurFunction := F;
-                Opsem.CurBB := B;
-                Opsem.CurCmds := c0 :: cs;
-                Opsem.Terminator := tmn;
-                Opsem.Locals := lc;
-                Opsem.Allocas := als |})
-  (Hwfcfg : OpsemPP.wf_Config cfg)
-  (Hwfpp : OpsemPP.wf_State cfg
-           {| Opsem.ECS := EC :: ECs;
-              Opsem.Mem := Mem0 |})
-  (Hnoalias : Promotability.wf_State maxb pinfo cfg
-           {| Opsem.ECS := EC :: ECs;
-              Opsem.Mem := Mem0 |})
-  (HwfS1 : wf_State pinfo alinfo cfg
-            {| Opsem.ECS := EC :: ECs;
-               Opsem.Mem := Mem0 |})
-  (Hnst : store_in_cmd (PI_id pinfo) c0 = false)
-  (Hneq :  F = PI_f pinfo ->
-           B = AI_block pinfo alinfo ->
-           id0 <> PI_id pinfo),
-  wf_State pinfo alinfo cfg
-     {|
-     Opsem.ECS := {|
-            Opsem.CurFunction := F;
-            Opsem.CurBB := B;
-            Opsem.CurCmds := cs;
-            Opsem.Terminator := tmn;
-            Opsem.Locals := updateAddAL (GVsT DGVs) lc id0 gv3;
-            Opsem.Allocas := als |} :: ECs;
-     Opsem.Mem := Mem0 |}.
-Proof.
-  intros. subst.
-  destruct cfg as [S [los nts] Ps gl fs].
-  destruct Hwfcfg as [_ [_ [HwfSystem HmInS]]].
-  destruct Hwfpp as 
-    [Hnonempty [
-     [Hreach1 [HBinF1 [HFinPs1 [_ [_ [l1 [ps1 [cs1' Heq1]]]]]]]]
-     [HwfEC0 HwfCall]
-    ]]; subst.
-  fold (@OpsemPP.wf_ECStack DGVs) in HwfEC0.
-
-  destruct HwfS1 as [Hinscope HwfECs]. simpl.
-  simpl in Hinscope, HwfECs.
-  fold wf_ECStack in HwfECs.
-
-  destruct Hnoalias as
-    [
-      [[Hinscope2' _] [HwfECs' _]]
-      [[Hdisjals _] HwfM]
-    ]. simpl in Hdisjals.
-  fold Promotability.wf_ECStack in HwfECs'.
-
-  split; auto.
-    intros J1 J2 J3. simpl in J1, J2, J3. simpl. subst.
-    unfold wf_ExecutionContext in *. simpl in Hinscope.
-    assert (uniqFdef (PI_f pinfo)) as Huniq. eauto using wf_system__uniqFdef.
-    assert (J2':=J2).
-    apply getCmdLoc_getCmdID in Hid; subst.
-    apply follow_alive_alloca_cons in J2; eauto.
-    assert (J2'':=J2).
-    apply Hinscope in J2; auto.
-    eapply wf_defs_updateAddAL; eauto.
-Qed.
-
-Lemma mstore_preserves_wf_EC_at_head: forall (maxb : Z) (pinfo : PhiInfo)
-  (alinfo : AllocaInfo pinfo) (S : system) los nts
-  (Ps : list product) (gl : GVMap) (fs : GVMap) (Hwfg : wf_globals maxb gl)
-  (F : fdef) (lc : Opsem.GVsMap) (sid : id) (t : typ) (align0 : align)
-  (v1 : value) (v2 : value) (cs : list cmd) (tmn : terminator) (Mem : mem)
-  (als : list mblock) (l1 : l) (ps1 : phinodes) (cs1' : list cmd)
-  (mp2 : GenericValue) (gv1 : GenericValue) (Mem' : mem) (gvs1 : GVsT DGVs)
-  (mps2 : GVsT DGVs) (Huniq: uniqFdef F)
-  (H : Opsem.getOperandValue (los,nts) v1 lc gl = ret gvs1)
-  (H0 : Opsem.getOperandValue (los,nts) v2 lc gl = ret mps2)
-  (Hwft: wf_value S (module_intro los nts Ps) F v2 (typ_pointer t))
-  (H1 : gv1 @ gvs1) (H2 : mp2 @ mps2) (Hwfpi: WF_PhiInfo pinfo)
-  (H3 : mstore (los,nts) Mem mp2 t gv1 align0 = ret Mem')
-  (Hinscope' : if fdef_dec (PI_f pinfo) F
-               then Promotability.wf_defs maxb pinfo (los,nts) Mem lc als
-               else True)
-  (HBinF: blockInFdefB (l1, stmts_intro ps1
-                          (cs1' ++ insn_store sid t v1 v2 align0 :: cs)
-                          tmn) F = true) (Huniq: uniqFdef F)
-  (Hinscope : wf_ExecutionContext pinfo alinfo (los,nts) Mem gl
-               {|
-               Opsem.CurFunction := F;
-               Opsem.CurBB := (l1, stmts_intro ps1
-                                (cs1' ++ insn_store sid t v1 v2 align0 :: cs)
-                                tmn);
-               Opsem.CurCmds := insn_store sid t v1 v2 align0 :: cs;
-               Opsem.Terminator := tmn;
-               Opsem.Locals := lc;
-               Opsem.Allocas := als |}),
-  wf_ExecutionContext pinfo alinfo (los,nts) Mem' gl
-     {|
-     Opsem.CurFunction := F;
-     Opsem.CurBB := (l1, stmts_intro ps1
-                      (cs1' ++ insn_store sid t v1 v2 align0 :: cs) tmn);
-     Opsem.CurCmds := cs;
-     Opsem.Terminator := tmn;
-     Opsem.Locals := lc;
-     Opsem.Allocas := als |}.
-Proof.
-  intros.
-  intros J1 J2 J3. simpl in J1, J2, J3. simpl. subst.
-  assert (J2':=J2).
-  remember (store_in_cmd (PI_id pinfo) (insn_store sid t v1 v2 align0)) as R.
-  destruct R.
-    clear - J2 J3 HeqR H3 H2 H0 H1 H.
-    unfold follow_alive_alloca in J3.
-    rewrite <- J2 in J3.
-    destruct alinfo. simpl in *.
-    assert (AI_alive0':=AI_alive0).
-    rewrite <- J2 in AI_alive0'.
-    destruct AI_alive0' as [G1 [G2 [cs1 [cs2 EQ]]]].
-    assert (EQ':=EQ).
-    apply J3 in EQ. clear J3.
-    destruct EQ as [csa [csb [EQ1 EQ2]]]; subst.
-    anti_simpl_env.
-    destruct csa.
-      anti_simpl_env. congruence.
-
-      assert (exists csa', exists c', [c] ++ csa = csa' ++ [c']) as EQ.
-        apply head_tail_commut.
-      destruct EQ as [csa' [c' EQ]].
-      simpl_env in EQ'.
-      rewrite EQ in EQ'.
-      anti_simpl_env. 
-      rewrite_env (([c] ++ csa) ++ csb) in G2.
-      rewrite EQ in G2.
-      simpl_env in G2.
-      apply store_in_cmds_app in G2.
-      destruct G2 as [G2 G3].
-      apply store_in_cmds_app in G3.
-      destruct G3 as [G3 G4].
-      unfold store_in_cmds in G3.
-      simpl in G3.
-      rewrite G3 in HeqR. congruence.
-
-    assert (getCmdLoc (insn_store sid t v1 v2 align0) <> PI_id pinfo) as Hneq.
-      apply WF_PhiInfo_spec10 in HBinF; auto.
-    apply follow_alive_alloca_cons in J2; auto.
-    apply Hinscope in J2; auto. simpl in J2.
-    destruct (fdef_dec (PI_f pinfo) (PI_f pinfo)); try congruence.
-    intros gvsa gvsv Hlkpa Hlkpv.
-    eapply J2 in Hlkpv; eauto.
-    eapply mstore_preserves_mload; eauto.
-      eapply operand__no_alias_with__head; eauto.
-        apply store_notin_cmd__wf_use_at_head in HeqR; auto.
-Qed.
-
-(* its proof is same to alive_store.v *)
-Lemma mstore_preserves_wf_EC_in_tail : forall pinfo los nts M EC M'
-  maxb gl (Hwfg: wf_globals maxb gl) lc v1 v2 gvs1 gv1 mps2 mp2 align0 t
-  (H : Opsem.getOperandValue (los,nts) v1 lc gl = ret gvs1)
-  (H0 : Opsem.getOperandValue (los,nts) v2 lc gl = ret mps2)
-  (H1 : gv1 @ gvs1) (H2 : mp2 @ mps2) F S Ps
-  (H3 : mstore (los,nts) M mp2 t gv1 align0 = ret M') alinfo
-  (Hinscope : wf_ExecutionContext pinfo alinfo (los,nts) M gl EC)
-  (Hwft: wf_value S (module_intro los nts Ps) F v2 (typ_pointer t))
-  (Hht : wf_ECStack_head_in_tail maxb pinfo (los,nts) M lc EC),
-  wf_ExecutionContext pinfo alinfo (los,nts) M' gl EC.
-Proof.
-  intros.
-  intros J1 J2 J3.
-  apply Hinscope in J3; auto.
-  intros gvsa gvsv Hlkpa Hlkpv.
-  eapply J3 in Hlkpv; eauto.
-  eapply mstore_preserves_mload; eauto.
-    eapply operand__no_alias_with__tail; eauto.
-Qed.
-
-(* its proof is same to alive_store.v *)
-Lemma mstore_preserves_wf_ECStack_in_tail : forall maxb pinfo los nts M
-  (Hwfpi: WF_PhiInfo pinfo) M' gl (Hwfg: wf_globals maxb gl)
-  maxb gl (Hwfg: wf_globals maxb gl) lc v1 v2 gvs1 gv1 mps2 mp2 align0 t
-  (H : Opsem.getOperandValue (los,nts) v1 lc gl = ret gvs1)
-  (H0 : Opsem.getOperandValue (los,nts) v2 lc gl = ret mps2)
-  (H1 : gv1 @ gvs1) (H2 : mp2 @ mps2)
-  (H3 : mstore (los,nts) M mp2 t gv1 align0 = ret M') stinfo
-  F S Ps
-  (Hwft: wf_value S (module_intro los nts Ps) F v2 (typ_pointer t)) ECs
-  (Hhts: wf_ECStack_head_tail maxb pinfo (los,nts) M lc ECs) 
-  (Hwf: wf_ECStack pinfo stinfo (los,nts) M gl ECs),
-  wf_ECStack pinfo stinfo (los,nts) M' gl ECs.
-Proof.
-  induction ECs; simpl; intros; auto.
-    destruct Hwf as [J1 J2].
-    apply wf_ECStack_head_tail_cons__inv in Hhts.
-    destruct Hhts as [J3 J4].
-    split; auto.
-      eapply mstore_preserves_wf_EC_in_tail with (gvs1:=gvs1)(mps2:=mps2)
-        in H3; eauto.
-Qed.
-
-(* same to alive_store.v *)
-Ltac preservation_malloc :=
-  destruct_ctx_other;
-  split; simpl; try solve [
-    eapply malloc_preserves_wf_EC_at_head;
-      eauto using wf_system__wf_fdef, wf_system__uniqFdef |
-    eapply malloc_preserves_wf_ECStack_in_tail; eauto].
-
-Lemma getOperandValue_updateAddAL_nouse: forall TD v lc rid v0 gl gvsv,
-  Opsem.getOperandValue TD v (updateAddAL (GVsT DGVs) lc rid v0) gl = ret gvsv ->
-  used_in_value rid v = false ->
-  Opsem.getOperandValue TD v lc gl = ret gvsv.
-Proof.
-  intros.
-  destruct v as [i0|]; simpl in *; auto.
-  rewrite <- lookupAL_updateAddAL_neq in H; auto.
-  destruct (id_dec i0 rid); auto.
-    simpl in H0. congruence.
-Qed.
-
-(* same to alive_store *)
-Lemma callExternalFunction_preserves_wf_EC_in_tail : forall pinfo td M EC M' gl
-  stinfo gvs fid oresult dck tr tret targs
-  (Hcall: callExternalOrIntrinsics td gl M fid tret targs dck gvs = 
-    ret (oresult, tr, M'))
-  (Hinscope : wf_ExecutionContext pinfo stinfo td M gl EC),
-  wf_ExecutionContext pinfo stinfo td M' gl EC.
-Proof.
-  intros.
-  intros J1 J2 J3.
-  apply Hinscope in J3; auto.
-  intros gvsa gvsv Hlkpa Hlkpv.
-  eapply J3 in Hlkpv; eauto.
-  eapply MemProps.callExternalOrIntrinsics_preserves_mload; eauto.
-Qed.
-
-(* same to alive_store *)
-Lemma callExternalFunction_preserves_wf_ECStack_in_tail: forall Mem fid gvs 
-  oresult Mem' pinfo stinfo TD gl ECs dck tret targs tr,
-  callExternalOrIntrinsics TD gl Mem fid tret targs dck gvs
-    = ret (oresult, tr, Mem') ->
-  wf_ECStack pinfo stinfo TD Mem gl ECs ->
-  wf_ECStack pinfo stinfo TD Mem' gl ECs.
-Proof.
-  induction ECs; simpl; intros; auto.
-    destruct H0.
-    split; eauto.
-      eapply callExternalFunction_preserves_wf_EC_in_tail; eauto.
-Qed.
-
-(* almost same to alive_store *)
-Lemma callExternalFunction_preserves_wf_ECStack_at_head: forall Mem fid gvs 
-  oresult Mem' pinfo stinfo gl rid noret0 ca rt1 va1 fv lp cs lc lc' als tmn
-  cs1' l1 ps1 F s los nts dck Ps (Hwfpi : WF_PhiInfo pinfo) tret targs tr
-  (HwfF: wf_fdef s (module_intro los nts Ps) F) (HuniqF: uniqFdef F)
-  (H4 : callExternalOrIntrinsics (los,nts) gl Mem fid tret targs dck gvs 
-          = ret (oresult, tr, Mem'))
-  (H5 : Opsem.exCallUpdateLocals (los,nts) rt1 noret0 rid oresult lc = ret lc')
-  (HBinF : blockInFdefB 
-             (l1, stmts_intro ps1 (cs1' ++ insn_call rid noret0 ca rt1 va1 fv lp :: cs) tmn)
-             F = true)
-  (Hinscope : wf_ExecutionContext pinfo stinfo (los,nts) Mem gl
-               {|
-               Opsem.CurFunction := F;
-               Opsem.CurBB := (l1, stmts_intro ps1
-                                (cs1' ++
-                                 insn_call rid noret0 ca rt1 va1 fv lp :: cs) tmn);
-               Opsem.CurCmds := insn_call rid noret0 ca rt1 va1 fv lp :: cs;
-               Opsem.Terminator := tmn;
-               Opsem.Locals := lc;
-               Opsem.Allocas := als |}),
-   wf_ExecutionContext pinfo stinfo (los,nts) Mem' gl
-     {|
-     Opsem.CurFunction := F;
-     Opsem.CurBB := (l1, stmts_intro ps1
-                      (cs1' ++ insn_call rid noret0 ca rt1 va1 fv lp :: cs) tmn);
-     Opsem.CurCmds := cs;
-     Opsem.Terminator := tmn;
-     Opsem.Locals := lc';
-     Opsem.Allocas := als |}.
-Proof.
-  intros.
-  intros J1 J2 J3. simpl in J1, J2, J3. simpl. subst.
-  assert (J2':=J2).
-  assert (rid <> PI_id pinfo) as Hneq.
-    eapply WF_PhiInfo_spec10 in HBinF; eauto.
-  apply follow_alive_alloca_cons in J2; auto.
-  apply Hinscope in J2; auto.
-  simpl in J2.
-  intros gvsa gvsv Hlka Hlkv.
-  unfold Opsem.exCallUpdateLocals in H5.
-  destruct noret0.
-    inv H5.
-    eapply J2 in Hlkv; eauto.
-    eapply MemProps.callExternalOrIntrinsics_preserves_mload; eauto.
-
-    destruct oresult; inv H5.
-    remember (fit_gv (los,nts) rt1 g) as R.
-    destruct R; inv H0.
-    rewrite <- lookupAL_updateAddAL_neq in Hlka; auto.
-    apply getOperandValue_updateAddAL_nouse in Hlkv; auto.
-    eapply MemProps.callExternalOrIntrinsics_preserves_mload; eauto.
-Qed.
-
-Ltac WF_PhiInfo_spec10_tac :=
-  match goal with
-  | HBinF1 : blockInFdefB (_, stmts_intro _ (_ ++ _ :: _) _) _ = true |- _ =>
-     eapply WF_PhiInfo_spec10 in HBinF1; eauto using wf_system__uniqFdef
-  end.
-
-Ltac preservation_pure_cmd_updated_case_helper:=
-  destruct_ctx_other;
-  intros; subst; WF_PhiInfo_spec10_tac.
-
-Ltac preservation_pure_cmd_updated_case:=
-  abstract (eapply preservation_pure_cmd_updated_case; eauto; try solve
-    [simpl; auto | preservation_pure_cmd_updated_case_helper]).
-
-Ltac free_preserves_wf_EC_at_head :=
-match goal with
-| Hinscope: wf_ExecutionContext ?pinfo _ _ _ _ _ |- _ =>
-  intros J1 J2 J3; simpl in J1, J2, J3; simpl; subst;
-  assert (J2':=J2);
-  apply follow_alive_alloca_cons in J2; eauto using wf_system__uniqFdef;
-    try solve [WF_PhiInfo_spec10_tac];
-  apply Hinscope in J2; auto; simpl in J2;
-  destruct (fdef_dec (PI_f pinfo) (PI_f pinfo)); try congruence;
-  intros gvsa gvsv Hlkpa Hlkpv;
-  eapply J2 in Hlkpv; eauto;
-  eapply free_preserves_mload; try solve [
-    eauto |
-    eapply operand__no_alias_with__head; try solve [
-      eauto | preservation_tac2 | get_wf_value_for_simop; eauto]
-    ]
-end.
 
 Lemma preservation : forall maxb pinfo alinfo cfg S1 S2 tr
   (Hwfg: wf_globals maxb (OpsemAux.Globals cfg))
@@ -916,72 +171,10 @@ Lemma preservation : forall maxb pinfo alinfo cfg S1 S2 tr
   (HwfS1: wf_State pinfo alinfo cfg S1), wf_State pinfo alinfo cfg S2.
 Proof.
   intros.
-  (sInsn_cases (induction HsInsn) Case); destruct TD as [los nts]; simpl HwfS1.
-
-Case "sReturn". abstract (eapply preservation_return; eauto).
-Case "sReturnVoid". abstract (eapply preservation_return_void; eauto).
-Case "sBranch". abstract preservation_sBranch.
-Case "sBranch_uncond". abstract preservation_sBranch.
-
-Case "sBop". preservation_pure_cmd_updated_case.
-Case "sFBop". preservation_pure_cmd_updated_case.
-Case "sExtractValue". preservation_pure_cmd_updated_case.
-Case "sInsertValue". preservation_pure_cmd_updated_case.
-
-Case "sMalloc". abstract preservation_malloc.
-
-Case "sFree".
-  abstract
-  (destruct_ctx_other;
-   split; simpl; try solve [
-    free_preserves_wf_EC_at_head |
-    eapply free_preserves_wf_ECStack_in_tail; try solve [
-      eauto | get_wf_value_for_simop; eauto]
-   ]).
-
-Case "sAlloca". abstract preservation_malloc.
-
-Case "sLoad". preservation_pure_cmd_updated_case.
-
-Case "sStore".
-   abstract
-   (destruct_ctx_other;
-    split; simpl; try solve [
-     eapply mstore_preserves_wf_EC_at_head; try solve [
-       eauto using wf_system__uniqFdef |
-       get_wf_value_for_simop; eauto
-     ] |
-     match goal with
-     | _ : ?gv1 @ ?gvs1', _ : ?mp2 @ ?mps2',
-       _ : mstore _ _ ?mp2 _ ?gv1 _ = _ |- _ =>
-       eapply mstore_preserves_wf_ECStack_in_tail
-         with (gvs1:=gvs1')(mps2:=mps2'); 
-         try solve [eauto | get_wf_value_for_simop; eauto]
-     end]).
-
-Case "sGEP". preservation_pure_cmd_updated_case.
-Case "sTrunc". preservation_pure_cmd_updated_case.
-Case "sExt". preservation_pure_cmd_updated_case.
-Case "sCast". preservation_pure_cmd_updated_case.
-Case "sIcmp". preservation_pure_cmd_updated_case.
-Case "sFcmp". preservation_pure_cmd_updated_case.
-Case "sSelect". destruct (isGVZero (los, nts) c); preservation_pure_cmd_updated_case.
-
-Case "sCall".
-  abstract (
-  destruct_ctx_other;
-  split; try solve [
-    intros J1 J2 J3; simpl in J1, J2, J3; simpl;
-    eapply follow_alive_alloca_at_beginning_false in J2; eauto; inv J2 |
-    split; auto]).
-
-Case "sExCall".
-  abstract (
-  destruct_ctx_other;
-  split; simpl; try solve [
-    eapply callExternalFunction_preserves_wf_ECStack_at_head; eauto using
-      wf_system__wf_fdef, wf_system__uniqFdef |
-    eapply callExternalFunction_preserves_wf_ECStack_in_tail; eauto]).
+  destruct (alinfo__minfo pinfo alinfo) as [minfo Heq].
+  eapply alinfo__wf_State__minfo; eauto.
+  eapply alinfo__wf_State__minfo in HwfS1; eauto.
+  eapply alive_mop.preservation; eauto.
 Qed.
 
 Lemma preservation_star : forall maxb pinfo alinfo cfg S1 S2 tr
@@ -1019,20 +212,8 @@ Lemma s_genInitState__alive_alloca: forall S main VarArgs cfg IS pinfo alinfo
   wf_State pinfo alinfo cfg IS.
 Proof.
   intros.
-  simpl_s_genInitState. 
-  split; simpl; auto.
-  unfold wf_ExecutionContext. simpl.
-  intros.
-  unfold wf_defs.
-  intros.
-  apply getParentOfFdefFromSystem__moduleInProductsInSystemB in HeqR0.
-  destruct HeqR0 as [J1 J2].
-  rewrite H in *.
-  eapply wf_system__uniqFdef in J1; eauto.
-  replace a with (getArgsOfFdef (PI_f pinfo)) in HeqR3.
-    erewrite WF_PhiInfo__pid_isnt_in_init in Hlkpa; eauto.
-    congruence.
-
-    rewrite <- H. auto.
+  destruct (alinfo__minfo pinfo alinfo) as [minfo Heq].
+  eapply alinfo__wf_State__minfo; eauto.
+  eapply alive_mop.s_genInitState__alive_mop; eauto.
 Qed.
 
