src3.0/Transforms/alive_store.v
@@ -11,6 +11,7 @@ Require Import primitives.
 Require Import palloca_props.
 Require Import memory_props.
 Require Import trans_tactic.
+Require Import alive_mop.
 
 Import Promotability.
 
@@ -34,6 +35,17 @@ exists cs1, exists cs3,
   cs2 ++
   cs3.
 
+Lemma alive_store__alive_mop: forall sid sal v (cs2:cmds) (b:block) (pinfo:PhiInfo)
+  (H: alive_store sid sal v cs2 b pinfo),
+  alive_mop v
+    (insn_store sid (PI_typ pinfo) v (value_id (PI_id pinfo)) sal) 
+    cs2 b pinfo.
+Proof.
+  intros. destruct b as [? []].
+  destruct H as [J1 [J2 [? [? ?]]]]; subst. 
+  unfold alive_mop. repeat (split; eauto). 
+Qed.
+
 Record StoreInfo (pinfo: PhiInfo) := mkStoreInfo {
   SI_id : id;
   SI_align : align;
@@ -43,20 +55,26 @@ Record StoreInfo (pinfo: PhiInfo) := mkStoreInfo {
   SI_alive : alive_store SI_id SI_align SI_value SI_tail SI_block pinfo
 }.
 
-Lemma storeinfo_doesnt_use_promotable_allocas: forall pinfo stinfo
-  (Huniq: uniqFdef (PI_f pinfo)),
-  WF_PhiInfo pinfo -> SI_value pinfo stinfo <> value_id (PI_id pinfo).
-Proof.
+Definition stinfo__eq__minfo pinfo stinfo minfo: Prop :=
+M_value pinfo minfo = SI_value pinfo stinfo /\
+M_c pinfo minfo = 
+   insn_store (SI_id pinfo stinfo) (PI_typ pinfo) (SI_value pinfo stinfo) 
+     (value_id (PI_id pinfo)) (SI_align pinfo stinfo) /\
+M_tail pinfo minfo = SI_tail pinfo stinfo /\
+M_block pinfo minfo = SI_block pinfo stinfo.
+
+Lemma stinfo__minfo: forall pinfo (stinfo: StoreInfo pinfo), 
+  { minfo: MopInfo pinfo | stinfo__eq__minfo pinfo stinfo minfo }.
+Proof.  
   intros.
-  destruct stinfo. simpl in *.
-  destruct SI_block0 as [? []].
-  destruct SI_alive0 as [J1 [J2 [cs1 [cs2 J3]]]]; subst.
-  eapply IngetCmdsIDs__lookupCmdViaIDFromFdef in J1; eauto using in_middle.
-    apply WF_PhiInfo_spec3 in J1; auto.
-    intro EQ; subst.
-    assert (G:=@valueEqB_refl (value_id (PI_id pinfo))).
-    destruct (valueEqB (value_id (PI_id pinfo)) (value_id (PI_id pinfo)));
-      simpl in *; try congruence.
+  destruct stinfo. 
+  exists (mkMopInfo pinfo SI_value0
+    (insn_store SI_id0 (PI_typ pinfo) SI_value0 (value_id (PI_id pinfo)) 
+      SI_align0)
+    SI_tail0 SI_block0 
+    (alive_store__alive_mop SI_id0 SI_align0 SI_value0 
+      SI_tail0 SI_block0 pinfo SI_alive0)).
+  split; auto.
 Qed.
 
 Definition wf_defs (pinfo:PhiInfo) (stinfo: StoreInfo pinfo) TD M gl (lc:DGVMap)
@@ -66,6 +84,15 @@ forall gvsa gvsv
   (Hlkpv: Opsem.getOperandValue TD (SI_value pinfo stinfo) lc gl
     = Some gvsv),
   mload TD M gvsa (PI_typ pinfo) (PI_align pinfo) = Some gvsv.
+
+Lemma stinfo__wf_defs__minfo: forall (pinfo:PhiInfo) stinfo
+  TD M gl (lc:DGVMap) minfo (Heq: stinfo__eq__minfo pinfo stinfo minfo),
+  wf_defs pinfo stinfo TD M gl lc <-> alive_mop.wf_defs pinfo minfo TD M gl lc.
+Proof.
+  intros. destruct Heq as [J1 [J2 [J3 J4]]].
+  unfold wf_defs, alive_mop.wf_defs.
+  rewrite J1. tauto.
+Qed.
 
 Definition follow_alive_store (pinfo:PhiInfo) (stinfo: StoreInfo pinfo)
   (cs:cmds) : Prop :=
@@ -80,44 +107,15 @@ forall cs1 cs3,
   (exists csa, exists csb,
     cs = csb ++ cs3 /\ SI_tail pinfo stinfo = csa ++ csb).
 
-Lemma follow_alive_store_cons: forall pinfo stinfo c cs l0 ps0 cs0 tmn0
-  (Huniq:uniqFdef (PI_f pinfo)),
-  (l0, stmts_intro ps0 (cs0++c::cs) tmn0) = SI_block pinfo stinfo ->
-  store_in_cmd (PI_id pinfo) c = false ->
-  follow_alive_store pinfo stinfo cs ->
-  follow_alive_store pinfo stinfo (c::cs).
+Lemma stinfo__follow_alive__minfo: forall (pinfo:PhiInfo) 
+  stinfo cs minfo 
+  (Heq: stinfo__eq__minfo pinfo stinfo minfo),
+  follow_alive_store pinfo stinfo cs <-> 
+    alive_mop.follow_alive_mop pinfo minfo cs.
 Proof.
-  unfold follow_alive_store.
-  intros.
-  destruct stinfo. simpl in *.
-  unfold alive_store in SI_alive0.
-  destruct SI_block0 as [? []].
-  destruct SI_alive0 as [J1 [J2 [cs1 [cs3 J3]]]]; subst.
-  intros.
-  assert (cs1 = cs2 /\ cs3 = cs4) as J.
-    eapply uniqFdef_cmds_split_middle in H2; eauto.
-    destruct H2 as [G1 G2].
-    split; auto.
-      apply app_inv_head in G2; auto.
-
-  destruct J as [EQ1 EQ2]; subst. clear H2.
-  edestruct H1 as [csa [csb [EQ1 EQ2]]]; eauto. clear H1.
-  subst. inv H.
-  anti_simpl_env.
-  destruct csa.
-    anti_simpl_env.
-    simpl in H0.
-    destruct (id_dec (PI_id pinfo) (PI_id pinfo)); simpl in H0; congruence.
-
-    assert (exists csa', exists c2, [c0] ++ csa = csa' ++ [c2]) as EQ.
-      apply head_tail_commut.
-    destruct EQ as [csa' [c2 EQ]].
-    simpl_env in H4.
-    rewrite EQ in H4. anti_simpl_env.
-    exists csa'. exists (c2::csb). simpl_env.
-    rewrite_env (([c0] ++ csa) ++ csb).
-    rewrite EQ. simpl_env.
-    split; auto.
+  intros. destruct Heq as [J1 [J2 [J3 J4]]].
+  unfold follow_alive_store, alive_mop.follow_alive_mop.
+  rewrite J4. rewrite J2. rewrite J3. tauto.
 Qed.
 
 Definition wf_ExecutionContext (pinfo:PhiInfo) (stinfo: StoreInfo pinfo) TD M gl
@@ -126,6 +124,23 @@ Opsem.CurFunction ec = PI_f pinfo ->
 Opsem.CurBB ec = SI_block pinfo stinfo ->
 follow_alive_store pinfo stinfo (Opsem.CurCmds ec) ->
 wf_defs pinfo stinfo TD M gl (Opsem.Locals ec).
+
+Lemma stinfo__wf_EC__minfo: forall (pinfo:PhiInfo) stinfo
+  TD M gl ec minfo (Heq: stinfo__eq__minfo pinfo stinfo minfo),
+  wf_ExecutionContext pinfo stinfo TD M gl ec <-> 
+    alive_mop.wf_ExecutionContext pinfo minfo TD M gl ec.
+Proof.
+  intros.
+  unfold wf_ExecutionContext, alive_mop.wf_ExecutionContext.
+  assert (J:=Heq).
+  apply stinfo__follow_alive__minfo with (cs:=Opsem.CurCmds ec) in J.
+  assert (J':=Heq).
+  apply stinfo__wf_defs__minfo with (lc:=Opsem.Locals ec)(TD:=TD)(M:=M)
+    (gl:=gl) in J'.
+  destruct Heq as [J1 [J2 [J3 J4]]].
+  rewrite J4.
+  tauto.
+Qed.
 
 Fixpoint wf_ECStack (pinfo:PhiInfo) (stinfo: StoreInfo pinfo) TD M gl
   (ecs:Opsem.ECStack) : Prop :=
@@ -136,106 +151,32 @@ match ecs with
     wf_ECStack pinfo stinfo TD M gl ecs'
 end.
 
+Lemma stinfo__wf_ECs__minfo: forall (pinfo:PhiInfo) stinfo
+  TD M gl minfo (Heq: stinfo__eq__minfo pinfo stinfo minfo) ecs,
+  wf_ECStack pinfo stinfo TD M gl ecs <-> 
+    alive_mop.wf_ECStack pinfo minfo TD M gl ecs.
+Proof.
+  induction ecs.
+    tauto.
+   
+    assert (J:=Heq).
+    apply stinfo__wf_EC__minfo with (ec:=a)(TD:=TD)(M:=M)(gl:=gl) in J.
+    simpl. tauto.
+Qed.
+
 Definition wf_State (pinfo:PhiInfo) (stinfo: StoreInfo pinfo)
   (cfg:OpsemAux.Config) (S:Opsem.State) : Prop :=
 wf_ECStack pinfo stinfo (OpsemAux.CurTargetData cfg) (Opsem.Mem S)
   (OpsemAux.Globals cfg) (Opsem.ECS S).
 
-Lemma free_allocas_preserves_wf_defs: forall pinfo TD Mem lc' als0 als Mem'
-  gl stinfo maxb,
-  Promotability.wf_defs maxb pinfo TD Mem lc' als0 ->
-  wf_defs pinfo stinfo TD Mem gl lc' ->
-  NoDup (als ++ als0) ->
-  free_allocas TD Mem als = ret Mem' ->
-  wf_defs pinfo stinfo TD Mem' gl lc'.
-Proof.
-  intros. unfold wf_defs in *. intros.
-  assert (Hlkpa':=Hlkpa).
-  eapply H0 in Hlkpa; eauto. clear H0.
-  eapply H in Hlkpa'; eauto.
-  destruct Hlkpa' as [J1 J2].
-  destruct J1 as [_ [[mb [J1 [J3 J4]]] _]]; subst.
-  eapply alist.NoDup_disjoint in H1; eauto.
-  eapply free_allocas_preserves_mload; eauto.
-Qed.
-
-Lemma wf_defs_updateAddAL: forall pinfo stinfo TD M lc' i1 gv1 gl
-  (Hwfpi: WF_PhiInfo pinfo) (Huniq: uniqFdef (PI_f pinfo))
-  (HwfDef: wf_defs pinfo stinfo TD M gl lc')
-  (Hneq: i1 <> PI_id pinfo)
-  (Hnouse: used_in_value i1 (SI_value pinfo stinfo) = false),
-  wf_defs pinfo stinfo TD M gl (updateAddAL _ lc' i1 gv1).
-Proof.
-  intros. unfold wf_defs in *. intros.
-  rewrite <- lookupAL_updateAddAL_neq in Hlkpa; auto.
-  eapply HwfDef; eauto.
-  apply storeinfo_doesnt_use_promotable_allocas with (stinfo:=stinfo) in Hwfpi;
-    auto.
-  destruct (SI_value pinfo stinfo) as [i0|]; simpl in *; auto.
-  destruct (id_dec i0 i1); simpl in Hnouse; try congruence.
-  rewrite <- lookupAL_updateAddAL_neq in Hlkpv; auto.
-Qed.
-
-Lemma free_allocas_preserves_wf_ECStack: forall maxb pinfo stinfo td als gl ECs
-  Mem Mem'
-  (HwfECs : Promotability.wf_ECStack maxb pinfo td Mem ECs)
-  (Hwfpi: WF_PhiInfo pinfo)
-  (Hndup: NoDup (als ++ (flat_map
-                  (fun ec : Opsem.ExecutionContext =>
-                   let '{| Opsem.Allocas := als |} := ec in als)
-                   ECs)))
-  (Hwf: wf_ECStack pinfo stinfo td Mem gl ECs)
-  (Hfrees: free_allocas td Mem als = ret Mem'),
-  wf_ECStack pinfo stinfo td Mem' gl ECs.
-Proof.
-  induction ECs as [|[]]; simpl; intros; auto.
-    destruct Hwf as [J1 J2].
-    assert (Hndup' := Hndup).
-    apply NoDup_strenthening in Hndup.
-    destruct HwfECs as [[Hwfdefs _] [HwfECs _]].
-    split; eauto.
-      intros G1 G2 G3. simpl in G1, G2, G3. subst. simpl.
-      apply J1 in G3; auto. simpl in G3.
-      destruct (fdef_dec (PI_f pinfo) (PI_f pinfo)); try congruence.
-      rewrite_env ((als ++ Allocas) ++
-        flat_map
-          (fun ec : Opsem.ExecutionContext =>
-           let '{| Opsem.Allocas := als |} := ec in als) ECs) in Hndup'.
-      apply NoDup_split in Hndup'. destruct Hndup'.
-      eapply free_allocas_preserves_wf_defs in G3; eauto.
-Qed.
-
-Lemma follow_alive_store_at_beginning_false: forall (pinfo : PhiInfo)
-  (stinfo : StoreInfo pinfo) (l' : l) (ps' : phinodes) (cs' : cmds)
-  (tmn' : terminator)
-  (J2 : (l', stmts_intro ps' cs' tmn') = SI_block pinfo stinfo)
-  (J3 : follow_alive_store pinfo stinfo cs'),
-  False.
+Lemma stinfo__wf_State__minfo: forall (pinfo:PhiInfo) stinfo
+  minfo (Heq: stinfo__eq__minfo pinfo stinfo minfo) cfg S,
+  wf_State pinfo stinfo cfg S <-> 
+    alive_mop.wf_State pinfo minfo cfg S.
 Proof.
   intros.
-  unfold follow_alive_store in J3.
-  rewrite <- J2 in J3.
-  destruct stinfo. simpl in *.
-  rewrite <- J2 in SI_alive0.
-  destruct SI_alive0 as [_ [_ [cs1 [cs3 J]]]].
-  assert (J':=J).
-  apply J3 in J.
-  destruct J as [csa [csb [EQ1 EQ2]]]; subst.
-  anti_simpl_env.
+  apply stinfo__wf_ECs__minfo; auto.
 Qed.
-
-Ltac preservation_sBranch :=
-match goal with
-| HwfS1 : wf_State _ _ _ _ |- _ =>
-  destruct HwfS1 as [_ HwfECs];
-  simpl in HwfECs;
-  fold wf_ECStack in HwfECs;
-  split; try solve [
-    auto |
-    intros J1 J2 J3; simpl in *; subst;
-    eapply follow_alive_store_at_beginning_false in J3; eauto;
-    inv J3]
-end.
 
 Ltac destruct_stinfo :=
 match goal with
@@ -247,761 +188,6 @@ match goal with
     [SI_BInF0 [SI_stincmds0 [SI_cs1 [SI_cs3 SI_EQ]]]]; subst; simpl
 end.
 
-Lemma alive_store_doesnt_use_its_followers_and_pid: forall l1 ps1 cs1' c cs tmn 
-  id0 pinfo stinfo s m (Huniq: uniqFdef (PI_f pinfo))
-  (Hreach: isReachableFromEntry (PI_f pinfo) 
-             (l1, stmts_intro ps1 (cs1' ++ c :: cs) tmn)),
-  wf_fdef s m (PI_f pinfo) -> 
-  (l1, stmts_intro ps1 (cs1' ++ c :: cs) tmn) = SI_block pinfo stinfo ->
-  getCmdID c = Some id0 ->
-  follow_alive_store pinfo stinfo (c::cs) ->
-  used_in_value id0 (SI_value pinfo stinfo) = false /\ id0 <> PI_id pinfo.
-Proof.
-  intros.
-Local Opaque isReachableFromEntry.
-  unfold follow_alive_store in H2.
-  rewrite <- H0 in H2.
-  destruct_stinfo. inv H0.
-  assert (J4':=H6).
-  apply_clear H2 in H6.
-  destruct H6 as [csa [csb [EQ1 EQ2]]]; subst.
-  rewrite EQ1 in J4'. 
-  anti_simpl_env. subst.
-  simpl in SI_BInF0.
-  assert (J1':=SI_BInF0).
-  eapply wf_fdef__wf_cmd in SI_BInF0; eauto using in_middle.
-  inv SI_BInF0.
-  match goal with | H13: wf_insn_base _ _ _ |- _ => inv H13 end.
-  assert (H0':=H0).
-  apply destruct_insnInFdefBlockB in H0'. destruct H0' as [HcInB HcInF].
-  rewrite <- EQ1 in *.
-  find_wf_operand_list.
-  match goal with
-  | H4: wf_operand_list _, H1: getCmdID _ = _ |- _ =>
-  eapply any_cmd_doesnt_use_following_operands 
-    with (c1:=insn_store SI_id0 (PI_typ pinfo) SI_value0
-                 (value_id (PI_id pinfo)) SI_align0)
-    (l3:=SI_l0)(ps1:=SI_ps0)
-    (c:=c)
-    (cs:=SI_cs1 ++
-             insn_store SI_id0 (PI_typ pinfo) SI_value0
-               (value_id (PI_id pinfo)) (SI_align0) :: 
-             csa ++ c :: cs)(tmn1:=SI_tmn0) in H4; eauto 1;
-    clear - H4 H1;
-    rewrite getCmdID__getCmdLoc with (id0:=id0) in H4; auto;
-    destruct SI_value0 as [i0|]; simpl in H4; simpl; try solve [
-      destruct (id_dec i0 id0); subst; try solve [
-        tauto |
-        destruct (id_dec id0 (PI_id pinfo)); subst; auto
-      ] |
-      destruct (id_dec id0 (PI_id pinfo)); subst; auto
-    ]
-  end.
-Qed.
-
-Lemma alive_store_doesnt_use_its_followers: forall l1 ps1 cs1' c cs tmn 
-  id0 pinfo stinfo s m (Huniq: uniqFdef (PI_f pinfo))
-  (Hreach: isReachableFromEntry (PI_f pinfo) 
-             (l1, stmts_intro ps1 (cs1' ++ c :: cs) tmn)),
-  wf_fdef s m (PI_f pinfo) -> 
-  (l1, stmts_intro ps1 (cs1' ++ c :: cs) tmn) = SI_block pinfo stinfo ->
-  getCmdID c = Some id0 ->
-  follow_alive_store pinfo stinfo (c::cs) ->
-  used_in_value id0 (SI_value pinfo stinfo) = false.
-Proof.
-  intros.
-  eapply alive_store_doesnt_use_its_followers_and_pid in H0; eauto.
-  tauto.
-Qed.
-
-Lemma preservation_return : forall maxb pinfo stinfo (HwfPI : WF_PhiInfo pinfo)
-  F B rid RetTy Result lc F' B' c' cs' tmn' lc' EC Mem als als' cfg
-  EC1 EC2
-  (EQ1:EC1 = {| Opsem.CurFunction := F;
-                Opsem.CurBB := B;
-                Opsem.CurCmds := nil;
-                Opsem.Terminator := insn_return rid RetTy Result;
-                Opsem.Locals := lc;
-                Opsem.Allocas := als |})
-  (EQ2:EC2 = {| Opsem.CurFunction := F';
-                Opsem.CurBB := B';
-                Opsem.CurCmds := c' :: cs';
-                Opsem.Terminator := tmn';
-                Opsem.Locals := lc';
-                Opsem.Allocas := als' |})
-  (Hwfcfg : OpsemPP.wf_Config cfg)  
-  (Hwfpp : OpsemPP.wf_State cfg
-           {| Opsem.ECS := EC1 :: EC2 :: EC;
-              Opsem.Mem := Mem |})
-  (Hnoalias : Promotability.wf_State maxb pinfo cfg
-           {| Opsem.ECS := EC1 :: EC2 :: EC;
-              Opsem.Mem := Mem |})
-  Mem' lc'' (H : Instruction.isCallInst c' = true)
-  (H0 : free_allocas (OpsemAux.CurTargetData cfg) Mem als = ret Mem')
-  (H1 : Opsem.returnUpdateLocals
-          (OpsemAux.CurTargetData cfg) c'
-            Result lc lc' (OpsemAux.Globals cfg) = ret lc'')
-  (HwfS1 : wf_State pinfo stinfo cfg
-            {| Opsem.ECS := EC1 :: EC2 :: EC;
-               Opsem.Mem := Mem |}),
-  wf_State pinfo stinfo cfg
-     {| Opsem.ECS :=
-             {| Opsem.CurFunction := F';
-                Opsem.CurBB := B';
-                Opsem.CurCmds := cs';
-                Opsem.Terminator := tmn';
-                Opsem.Locals := lc'';
-                Opsem.Allocas := als' |} :: EC;
-        Opsem.Mem := Mem' |}.
-Proof.
-  intros. subst. destruct cfg as [S [los nts] Ps gl fs].
-
-  destruct Hwfcfg as [_ [_ [HwfSystem HmInS]]].
-  destruct Hwfpp as 
-    [_ [_ 
-     [
-       [
-         [Hreach1 [HBinF1 [HFinPs1 [_ [_ [l2 [ps2 [cs2' Heq2]]]]]]]]
-         _
-       ]
-       _
-     ]
-    ]]; subst.
-
-  destruct HwfS1 as [Hinscope1 [Hinscope2 HwfECs]]. simpl.
-  simpl in Hinscope1, Hinscope2, HwfECs.
-  fold wf_ECStack in HwfECs.
-
-  destruct Hnoalias as
-    [
-      [_ [[[Hinscope2' _] [HwfECs' _]] _]]
-      [[Hdisjals _] HwfM]
-    ]. simpl in Hdisjals.
-  fold Promotability.wf_ECStack in HwfECs'.
-
-  split.
-    SSCase "wf_EC".
-    intros J1 J2 J3. simpl in J1, J2, J3. simpl. subst.
-    remember (getCmdID c') as R.
-    destruct_cmd c'; try solve [inversion H].
-    unfold wf_ExecutionContext in *. simpl in Hinscope1, Hinscope2.
-    assert (J2':=J2).
-    assert (uniqFdef (PI_f pinfo)) as Huniq. eauto using wf_system__uniqFdef.
-    apply follow_alive_store_cons in J2; auto.
-    assert (J2'':=J2).
-    apply Hinscope2 in J2; auto.
-    assert (NoDup (als ++ als')) as Hnodup.
-      rewrite_env
-        ((als ++ als') ++
-          flat_map
-            (fun ec : Opsem.ExecutionContext =>
-             let '{| Opsem.Allocas := als |} := ec in als) EC) in Hdisjals.
-      apply NoDup_split in Hdisjals.
-      destruct Hdisjals; auto.
-    destruct (fdef_dec (PI_f pinfo) (PI_f pinfo)); try congruence.
-    eapply free_allocas_preserves_wf_defs in J2; eauto. clear Hnodup.
-      unfold Opsem.returnUpdateLocals in H1. simpl in H1.
-      remember (Opsem.getOperandValue (los,nts) Result lc gl) as R1.
-      destruct R1; try solve [inv H1].
-      destruct R.
-      SSSSSCase "c' defines a variable".
-        destruct n; inv HeqR.
-        remember (lift_op1 DGVs (fit_gv (los, nts) t0) g t0) as R2.
-        destruct R2; inv H1.
-        apply wf_defs_updateAddAL; auto.
-          eapply WF_PhiInfo_spec10 in HBinF1; eauto.
-          eapply alive_store_doesnt_use_its_followers;
-            eauto using wf_system__wf_fdef.
-
-      SSSSSCase "c' defines nothing".
-        destruct n; inv HeqR. inv H1. auto.
-
-    SSCase "wf_ECs".
-      simpl.
-      eapply free_allocas_preserves_wf_ECStack; eauto.
-      apply NoDup_strenthening in Hdisjals; auto.
-Qed.
-
-Lemma preservation_return_void : forall maxb pinfo stinfo
-  (HwfPI : WF_PhiInfo pinfo)
-  F B rid lc F' B' c' cs' tmn' lc' EC Mem als als' cfg EC1 EC2
-  (EQ1:EC1 = {| Opsem.CurFunction := F;
-                Opsem.CurBB := B;
-                Opsem.CurCmds := nil;
-                Opsem.Terminator := insn_return_void rid;
-                Opsem.Locals := lc;
-                Opsem.Allocas := als |})
-  (EQ2:EC2 = {| Opsem.CurFunction := F';
-                Opsem.CurBB := B';
-                Opsem.CurCmds := c' :: cs';
-                Opsem.Terminator := tmn';
-                Opsem.Locals := lc';
-                Opsem.Allocas := als' |})
-  (Hwfcfg : OpsemPP.wf_Config cfg)
-  (Hwfpp : OpsemPP.wf_State cfg
-           {| Opsem.ECS := EC1 :: EC2 :: EC;
-              Opsem.Mem := Mem |})
-  (Hnoalias : Promotability.wf_State maxb pinfo cfg
-           {| Opsem.ECS := EC1 :: EC2 :: EC;
-              Opsem.Mem := Mem |})
-  Mem' (H : Instruction.isCallInst c' = true)
-  (H0 : free_allocas (OpsemAux.CurTargetData cfg) Mem als = ret Mem')
-  (HwfS1 : wf_State pinfo stinfo cfg
-            {| Opsem.ECS := EC1 :: EC2 :: EC;
-               Opsem.Mem := Mem |}),
-  wf_State pinfo stinfo cfg
-     {| Opsem.ECS :=
-             {| Opsem.CurFunction := F';
-                Opsem.CurBB := B';
-                Opsem.CurCmds := cs';
-                Opsem.Terminator := tmn';
-                Opsem.Locals := lc';
-                Opsem.Allocas := als' |} :: EC;
-        Opsem.Mem := Mem' |}.
-Proof.
-  intros. subst. destruct cfg as [S [los nts] Ps gl fs].
-  destruct Hwfcfg as [_ [_ [HwfSystem HmInS]]].
-  destruct Hwfpp as 
-    [_ [_ 
-     [
-       [
-         [Hreach1 [HBinF1 [HFinPs1 [_ [_ [l2 [ps2 [cs2' Heq2]]]]]]]]
-         _
-       ]
-       _
-     ]
-    ]]; subst.
-
-  destruct HwfS1 as [Hinscope1 [Hinscope2 HwfECs]]. simpl.
-  simpl in Hinscope1, Hinscope2, HwfECs.
-  fold wf_ECStack in HwfECs.
-
-  destruct Hnoalias as
-    [
-      [_ [[[Hinscope2' _] [HwfECs' _]] _]]
-      [[Hdisjals _] HwfM]
-    ]. simpl in Hdisjals.
-  fold Promotability.wf_ECStack in HwfECs'.
-
-  split.
-    SSCase "wf_EC".
-    intros J1 J2 J3. simpl in J1, J2, J3. simpl. subst.
-    remember (getCmdID c') as R.
-    destruct c'; try solve [inversion H].
-    unfold wf_ExecutionContext in *. simpl in Hinscope1, Hinscope2.
-    assert (J2':=J2).
-    apply follow_alive_store_cons in J2; eauto using wf_system__uniqFdef.
-    apply Hinscope2 in J2; auto.
-    assert (NoDup (als ++ als')) as Hnodup.
-      rewrite_env
-        ((als ++ als') ++
-          flat_map
-            (fun ec : Opsem.ExecutionContext =>
-             let '{| Opsem.Allocas := als |} := ec in als) EC) in Hdisjals.
-      apply NoDup_split in Hdisjals.
-      destruct Hdisjals; auto.
-    destruct (fdef_dec (PI_f pinfo) (PI_f pinfo)); try congruence.
-    eapply free_allocas_preserves_wf_defs in J2; eauto.
-
-    SSCase "wf_ECs".
-      simpl.
-      eapply free_allocas_preserves_wf_ECStack; eauto.
-      apply NoDup_strenthening in Hdisjals; auto.
-Qed.
-
-Lemma malloc_preserves_wf_EC_at_head : forall pinfo los nts Ps M
-  (Hwfpi:WF_PhiInfo pinfo) s als'
-  M' gl als lc t mb id0 align0 F gn tsz l1 ps1 cs1' cs tmn
-  (HwfF: wf_fdef s (module_intro los nts Ps) F) (HuniqF: uniqFdef F)
-  (Hal: malloc (los,nts) M tsz gn align0 = ret (M', mb)) stinfo c
-  (HBinF: blockInFdefB
-             (l1, stmts_intro ps1 (cs1' ++ c :: cs)
-                tmn) F = true)
-  (Hid : getCmdID c = Some id0)
-  (Hnst : store_in_cmd (PI_id pinfo) c = false)
-  (Hsort : match c with
-           | insn_malloc _ _ _ _ | insn_alloca _ _ _ _ => True
-           | _ => False
-           end)
-  (Hreach: isReachableFromEntry F
-             (l1, stmts_intro ps1 (cs1' ++ c :: cs) tmn))
-  (Hinscope : wf_ExecutionContext pinfo stinfo (los,nts) M gl
-               {|
-               Opsem.CurFunction := F;
-               Opsem.CurBB := (l1, stmts_intro ps1
-                                (cs1' ++ c :: cs)
-                                tmn);
-               Opsem.CurCmds := c :: cs;
-               Opsem.Terminator := tmn;
-               Opsem.Locals := lc;
-               Opsem.Allocas := als |}),
-  wf_ExecutionContext pinfo stinfo (los,nts) M' gl
-    {|
-    Opsem.CurFunction := F;
-    Opsem.CurBB := (l1, stmts_intro ps1
-                      (cs1' ++ c :: cs) tmn);
-    Opsem.CurCmds := cs;
-    Opsem.Terminator := tmn;
-    Opsem.Locals := updateAddAL (GVsT DGVs) lc id0
-                       ($ blk2GV (los,nts) mb # typ_pointer t $);
-    Opsem.Allocas := als' |}.
-Proof.
-  intros.
-  intros J1 J2 J3. simpl in J1, J2, J3. simpl. subst.
-  assert (J2':=J2).
-  apply follow_alive_store_cons in J2; auto.
-  assert (Hfollow:=J2).
-  assert (used_in_value id0 (SI_value pinfo stinfo) = false) as Hnuse.
-    eapply alive_store_doesnt_use_its_followers; eauto.
-  apply Hinscope in J2; auto. simpl in J2.
-  destruct (fdef_dec (PI_f pinfo) (PI_f pinfo)); try congruence.
-  apply wf_defs_updateAddAL with (i1:=id0)
-    (gv1:=($ blk2GV (los,nts) mb # typ_pointer t $)) in J2; auto.
-    intros gvsa gvsv Hlkpa Hlkpv.
-    eapply J2 in Hlkpv; eauto.
-    eapply malloc_preserves_mload; eauto.
-      destruct (id_dec id0 (PI_id pinfo)); subst; auto.
-      destruct_cmd c; tinv Hsort.
-        apply getCmdLoc_getCmdID in Hid; subst.
-        eapply WF_PhiInfo_spec10 in HBinF; eauto.
-
-        inv Hid.
-        eapply alive_store_doesnt_use_its_followers_and_pid in J2'; simpl; eauto.
-Qed.
-
-Lemma malloc_preserves_wf_EC_in_tail : forall pinfo td M
-  EC M' gl mb align0 gn tsz
-  (Hal: malloc td M tsz gn align0 = ret (M', mb)) stinfo
-  (Hinscope : wf_ExecutionContext pinfo stinfo td M gl EC),
-  wf_ExecutionContext pinfo stinfo td M' gl EC.
-Proof.
-  intros.
-  intros J1 J2 J3.
-  apply Hinscope in J3; auto.
-  intros gvsa gvsv Hlkpa Hlkpv.
-  eapply J3 in Hlkpv; eauto.
-  eapply malloc_preserves_mload; eauto.
-Qed.
-
-Lemma malloc_preserves_wf_ECStack_in_tail : forall pinfo stinfo TD M tsz gn
-  align0 (Hwfpi: WF_PhiInfo pinfo) M' mb gl
-  (Hmlc: malloc TD M tsz gn align0 = ret (M', mb)) ECs
-  (Hwf: wf_ECStack pinfo stinfo TD M gl ECs),
-  wf_ECStack pinfo stinfo TD M' gl ECs.
-Proof.
-  induction ECs; simpl; intros; auto.
-    destruct Hwf as [J1 J2].
-    split; auto.
-      eapply malloc_preserves_wf_EC_in_tail; eauto.
-Qed.
-
-Lemma free_preserves_wf_EC_in_tail : forall pinfo los nts M EC M' mptr0
-  maxb gl (Hwfg: wf_globals maxb gl) Ps S F t
-  (Hfree: free (los,nts) M mptr0 = ret M') stinfo mptrs v lc
-  (Hwft: wf_value S (module_intro los nts Ps) F v t)
-  (H : Opsem.getOperandValue (los,nts) v lc gl = ret mptrs)
-  (H0 : mptr0 @ mptrs)
-  (Hinscope : wf_ExecutionContext pinfo stinfo (los,nts) M gl EC)
-  (Hht : wf_ECStack_head_in_tail maxb pinfo (los,nts) M lc EC),
-  wf_ExecutionContext pinfo stinfo (los,nts) M' gl EC.
-Proof.
-  intros.
-  intros J1 J2 J3.
-  apply Hinscope in J3; auto.
-  intros gvsa gvsv Hlkpa Hlkpv.
-  eapply J3 in Hlkpv; eauto.
-  eapply free_preserves_mload; eauto.
-    eapply operand__no_alias_with__tail; eauto.
-Qed.
-
-Lemma free_preserves_wf_ECStack_in_tail : forall maxb pinfo stinfo los nts M
-  (Hwfpi: WF_PhiInfo pinfo) M' gl mptr0 (Hwfg: wf_globals maxb gl)
-  (Hfree: free (los,nts) M mptr0 = ret M') lc mptrs v t S Ps F
-  (Hwft: wf_value S (module_intro los nts Ps) F v t)
-  (H : Opsem.getOperandValue (los,nts) v lc gl = ret mptrs)
-  (H0 : mptr0 @ mptrs) ECs
-  (Hhts: wf_ECStack_head_tail maxb pinfo (los,nts) M lc ECs)
-  (Hwf: wf_ECStack pinfo stinfo (los,nts) M gl ECs),
-  wf_ECStack pinfo stinfo (los,nts) M' gl ECs.
-Proof.
-  induction ECs; simpl; intros; auto.
-    destruct Hwf as [J1 J2].
-    apply wf_ECStack_head_tail_cons__inv in Hhts.
-    destruct Hhts as [J3 J4].
-    split; auto.
-      eapply free_preserves_wf_EC_in_tail; eauto.
-Qed.
-
-Lemma preservation_pure_cmd_updated_case : forall (F : fdef)(B : block)
-  (lc : DGVMap)(gv3 : GVsT DGVs) (cs : list cmd) (tmn : terminator) id0 c0 Mem0
-  als ECs pinfo stinfo
-  (HwfPI : WF_PhiInfo pinfo) (Hid : Some id0 = getCmdID c0) cfg maxb EC
-  (Heq: EC = {| Opsem.CurFunction := F;
-                Opsem.CurBB := B;
-                Opsem.CurCmds := c0 :: cs;
-                Opsem.Terminator := tmn;
-                Opsem.Locals := lc;
-                Opsem.Allocas := als |})
-  (Hwfcfg : OpsemPP.wf_Config cfg)
-  (Hwfpp : OpsemPP.wf_State cfg
-           {| Opsem.ECS := EC :: ECs;
-              Opsem.Mem := Mem0 |})
-  (Hnoalias : Promotability.wf_State maxb pinfo cfg
-           {| Opsem.ECS := EC :: ECs;
-              Opsem.Mem := Mem0 |})
-  (HwfS1 : wf_State pinfo stinfo cfg
-            {| Opsem.ECS := EC :: ECs;
-               Opsem.Mem := Mem0 |})
-  (Hnst : store_in_cmd (PI_id pinfo) c0 = false)
-  (Hneq :  F = PI_f pinfo ->
-           B = SI_block pinfo stinfo ->
-           follow_alive_store pinfo stinfo (c0 :: cs) ->
-           (id0 <> PI_id pinfo /\
-           used_in_value id0 (SI_value pinfo stinfo) = false)),
-  wf_State pinfo stinfo cfg
-     {|
-     Opsem.ECS := {|
-            Opsem.CurFunction := F;
-            Opsem.CurBB := B;
-            Opsem.CurCmds := cs;
-            Opsem.Terminator := tmn;
-            Opsem.Locals := updateAddAL (GVsT DGVs) lc id0 gv3;
-            Opsem.Allocas := als |} :: ECs;
-     Opsem.Mem := Mem0 |}.
-Proof.
-  intros. subst.
-  destruct cfg as [S [los nts] Ps gl fs].
-  destruct Hwfcfg as [_ [_ [HwfSystem HmInS]]].
-  destruct Hwfpp as 
-    [Hnonempty [
-     [Hreach1 [HBinF1 [HFinPs1 [_ [_ [l1 [ps1 [cs1' Heq1]]]]]]]]
-     [HwfEC0 HwfCall]
-    ]]; subst.
-  fold (@OpsemPP.wf_ECStack DGVs) in HwfEC0.
-
-  destruct HwfS1 as [Hinscope HwfECs]. simpl.
-  simpl in Hinscope, HwfECs.
-  fold wf_ECStack in HwfECs.
-
-  destruct Hnoalias as
-    [
-      [[Hinscope2' _] [HwfECs' _]]
-      [[Hdisjals _] HwfM]
-    ]. simpl in Hdisjals.
-  fold Promotability.wf_ECStack in HwfECs'.
-
-  split; auto.
-    intros J1 J2 J3. simpl in J1, J2, J3. simpl. subst.
-    unfold wf_ExecutionContext in *. simpl in Hinscope.
-    assert (uniqFdef (PI_f pinfo)) as Huniq. eauto using wf_system__uniqFdef.
-    assert (J2':=J2).
-    apply follow_alive_store_cons in J2; auto.
-    assert (J2'':=J2).
-    apply Hinscope in J2; auto.
-    destruct Hneq as [G1 G2]; auto.
-    eapply wf_defs_updateAddAL; eauto.
-Qed.
-
-Lemma mstore_preserves_wf_EC_at_head: forall (maxb : Z) (pinfo : PhiInfo)
-  (stinfo : StoreInfo pinfo) (S : system) los nts
-  (Ps : list product) (gl : GVMap) (fs : GVMap) (Hwfg : wf_globals maxb gl)
-  (F : fdef) (lc : Opsem.GVsMap) (sid : id) (t : typ) (align0 : align)
-  (v1 : value) (v2 : value) (cs : list cmd) (tmn : terminator) (Mem : mem)
-  (als : list mblock) (l1 : l) (ps1 : phinodes) (cs1' : list cmd)
-  (mp2 : GenericValue) (gv1 : GenericValue) (Mem' : mem) (gvs1 : GVsT DGVs)
-  (mps2 : GVsT DGVs) (Huniq: uniqFdef F)
-  (H : Opsem.getOperandValue (los,nts) v1 lc gl = ret gvs1)
-  (H0 : Opsem.getOperandValue (los,nts) v2 lc gl = ret mps2)
-  (Hwft2: wf_value S (module_intro los nts Ps) F v2 (typ_pointer t))
-  (Hwft1: wf_value S (module_intro los nts Ps) F v1 t)
-  (Hwfgl: genericvalues.LLVMgv.wf_global (los, nts) S gl)
-  (H1 : gv1 @ gvs1) (H2 : mp2 @ mps2)
-  (H3 : mstore (los,nts) Mem mp2 t gv1 align0 = ret Mem')
-  (Hwflc: OpsemPP.wf_lc (los,nts) F lc)
-  (Hinscope' : if fdef_dec (PI_f pinfo) F
-               then Promotability.wf_defs maxb pinfo (los,nts) Mem lc als
-               else True)
-  (Hinscope : wf_ExecutionContext pinfo stinfo (los,nts) Mem gl
-               {|
-               Opsem.CurFunction := F;
-               Opsem.CurBB := (l1, stmts_intro ps1
-                                (cs1' ++ insn_store sid t v1 v2 align0 :: cs)
-                                tmn);
-               Opsem.CurCmds := insn_store sid t v1 v2 align0 :: cs;
-               Opsem.Terminator := tmn;
-               Opsem.Locals := lc;
-               Opsem.Allocas := als |}),
-  wf_ExecutionContext pinfo stinfo (los,nts) Mem' gl
-     {|
-     Opsem.CurFunction := F;
-     Opsem.CurBB := (l1, stmts_intro ps1
-                      (cs1' ++ insn_store sid t v1 v2 align0 :: cs) tmn);
-     Opsem.CurCmds := cs;
-     Opsem.Terminator := tmn;
-     Opsem.Locals := lc;
-     Opsem.Allocas := als |}.
-Proof.
-  intros.
-  intros J1 J2 J3. simpl in J1, J2, J3. simpl. subst.
-  assert (J2':=J2).
-  remember (store_in_cmd (PI_id pinfo) (insn_store sid t v1 v2 align0)) as R.
-  destruct R.
-    clear - J2 J3 HeqR H3 H2 H0 H1 H Hwflc Hwft1 Hwfgl.
-    unfold follow_alive_store in J3.
-    rewrite <- J2 in J3.
-    destruct stinfo. simpl in *.
-    assert (SI_alive0':=SI_alive0).
-    rewrite <- J2 in SI_alive0'.
-    destruct SI_alive0' as [G1 [G2 [cs1 [cs2 EQ]]]].
-    assert (EQ':=EQ).
-    apply J3 in EQ. clear J3.
-    destruct EQ as [csa [csb [EQ1 EQ2]]]; subst.
-    anti_simpl_env. 
-    destruct csa.
-      simpl_env in EQ'.
-      apply app_inj_tail in EQ'.
-      destruct EQ' as [EQ1 EQ2]; subst.
-      inv EQ2.
-      intros gvsa gvsv Hlkpa Hlkpv.
-      simpl in *.
-      rewrite H0 in Hlkpa. inv Hlkpa. inv H2. inv H1.
-      rewrite Hlkpv in H. inv H.
-      eapply MemProps.mstore_mload_same; eauto.
-        eapply OpsemPP.getOperandValue__wf_gvs in Hlkpv; eauto.
-        inv Hlkpv; eauto.
-
-      assert (exists csa', exists c', [c] ++ csa = csa' ++ [c']) as EQ.
-        apply head_tail_commut.
-      destruct EQ as [csa' [c' EQ]].
-      simpl_env in EQ'.
-      rewrite EQ in EQ'.
-      anti_simpl_env. rewrite_env (([c]++csa) ++ csb) in G2.
-      rewrite EQ in G2.
-      simpl_env in G2.
-      apply store_in_cmds_app in G2.
-      destruct G2 as [G2 G3].
-      apply store_in_cmds_app in G3.
-      destruct G3 as [G3 G4].
-      unfold store_in_cmds in G3.
-      simpl in G3.
-      rewrite G3 in HeqR. congruence.
-
-    clear Hwft1 Hwfgl.
-    apply follow_alive_store_cons in J2; auto.
-    apply Hinscope in J2; auto. simpl in J2.
-    destruct (fdef_dec (PI_f pinfo) (PI_f pinfo)); try congruence.
-    intros gvsa gvsv Hlkpa Hlkpv.
-    eapply J2 in Hlkpv; eauto.
-    eapply mstore_preserves_mload; eauto.
-      eapply operand__no_alias_with__head; eauto.
-        apply store_notin_cmd__wf_use_at_head in HeqR; auto.
-Qed.
-
-Lemma mstore_preserves_wf_EC_in_tail : forall pinfo los nts M EC M'
-  maxb gl (Hwfg: wf_globals maxb gl) lc v1 v2 gvs1 gv1 mps2 mp2 align0 t
-  (H : Opsem.getOperandValue (los,nts) v1 lc gl = ret gvs1)
-  (H0 : Opsem.getOperandValue (los,nts) v2 lc gl = ret mps2)
-  (H1 : gv1 @ gvs1) (H2 : mp2 @ mps2) F S Ps
-  (H3 : mstore (los,nts) M mp2 t gv1 align0 = ret M') stinfo
-  (Hinscope : wf_ExecutionContext pinfo stinfo (los,nts) M gl EC)
-  (Hwft: wf_value S (module_intro los nts Ps) F v2 (typ_pointer t))
-  (Hht : wf_ECStack_head_in_tail maxb pinfo (los,nts) M lc EC),
-  wf_ExecutionContext pinfo stinfo (los,nts) M' gl EC.
-Proof.
-  intros.
-  intros J1 J2 J3.
-  apply Hinscope in J3; auto.
-  intros gvsa gvsv Hlkpa Hlkpv.
-  eapply J3 in Hlkpv; eauto.
-  eapply mstore_preserves_mload; eauto.
-    eapply operand__no_alias_with__tail; eauto.
-Qed.
-
-Lemma mstore_preserves_wf_ECStack_in_tail : forall maxb pinfo los nts M
-  (Hwfpi: WF_PhiInfo pinfo) M' gl (Hwfg: wf_globals maxb gl)
-  maxb gl (Hwfg: wf_globals maxb gl) lc v1 v2 gvs1 gv1 mps2 mp2 align0 t
-  (H : Opsem.getOperandValue (los,nts) v1 lc gl = ret gvs1)
-  (H0 : Opsem.getOperandValue (los,nts) v2 lc gl = ret mps2)
-  (H1 : gv1 @ gvs1) (H2 : mp2 @ mps2)
-  (H3 : mstore (los,nts) M mp2 t gv1 align0 = ret M') stinfo
-  F S Ps
-  (Hwft: wf_value S (module_intro los nts Ps) F v2 (typ_pointer t)) ECs
-  (Hhts: wf_ECStack_head_tail maxb pinfo (los,nts) M lc ECs) 
-  (Hwf: wf_ECStack pinfo stinfo (los,nts) M gl ECs),
-  wf_ECStack pinfo stinfo (los,nts) M' gl ECs.
-Proof.
-  induction ECs; simpl; intros; auto.
-    destruct Hwf as [J1 J2].
-    apply wf_ECStack_head_tail_cons__inv in Hhts.
-    destruct Hhts as [J3 J4].
-    split; auto.
-      eapply mstore_preserves_wf_EC_in_tail with (gvs1:=gvs1)(mps2:=mps2)
-        in H3; eauto.
-Qed.
-
-Lemma getOperandValue_updateAddAL_nouse: forall TD v lc rid v0 gl gvsv,
-  Opsem.getOperandValue TD v (updateAddAL (GVsT DGVs) lc rid v0) gl = ret gvsv ->
-  used_in_value rid v = false ->
-  Opsem.getOperandValue TD v lc gl = ret gvsv.
-Proof.
-  intros.
-  destruct v as [i0|]; simpl in *; auto.
-  rewrite <- lookupAL_updateAddAL_neq in H; auto.
-  destruct (id_dec i0 rid); auto.
-    simpl in H0. congruence.
-Qed.
-
-Lemma callExternalFunction_preserves_wf_EC_in_tail : forall pinfo td M EC M' gl
-  stinfo gvs fid oresult dck tret targs tr
-  (Hcall: callExternalOrIntrinsics td gl M fid tret targs dck gvs = 
-    ret (oresult, tr, M'))
-  (Hinscope : wf_ExecutionContext pinfo stinfo td M gl EC),
-  wf_ExecutionContext pinfo stinfo td M' gl EC.
-Proof.
-  intros.
-  intros J1 J2 J3.
-  apply Hinscope in J3; auto.
-  intros gvsa gvsv Hlkpa Hlkpv.
-  eapply J3 in Hlkpv; eauto.
-  eapply MemProps.callExternalOrIntrinsics_preserves_mload; eauto.
-Qed.
-
-Lemma callExternalFunction_preserves_wf_ECStack_in_tail: forall Mem fid gvs
-  oresult Mem' pinfo stinfo TD gl ECs dck tret targs tr,
-  callExternalOrIntrinsics TD gl Mem fid tret targs dck gvs = 
-    ret (oresult, tr, Mem') ->
-  wf_ECStack pinfo stinfo TD Mem gl ECs ->
-  wf_ECStack pinfo stinfo TD Mem' gl ECs.
-Proof.
-  induction ECs; simpl; intros; auto.
-    destruct H0.
-    split; eauto.
-      eapply callExternalFunction_preserves_wf_EC_in_tail; eauto.
-Qed.
-
-Lemma callExternalFunction_preserves_wf_ECStack_at_head: forall Mem fid gvs
-  oresult Mem' pinfo stinfo gl rid noret0 ca rt1 va1 fv lp cs lc lc' als tmn
-  cs1' l1 ps1 F s los nts dck Ps (Hwfpi : WF_PhiInfo pinfo) tret targs tr
-  (HwfF: wf_fdef s (module_intro los nts Ps) F) (HuniqF: uniqFdef F)
-  (H4 : callExternalOrIntrinsics (los,nts) gl Mem fid tret targs dck gvs 
-          = ret (oresult, tr, Mem'))
-  (H5 : Opsem.exCallUpdateLocals (los,nts) rt1 noret0 rid oresult lc = ret lc')
-  (HBinF : blockInFdefB 
-             (l1, stmts_intro ps1 
-               (cs1' ++ insn_call rid noret0 ca rt1 va1 fv lp :: cs) tmn)
-             F = true)
-  (Hreach: isReachableFromEntry F
-             (l1, stmts_intro ps1 
-               (cs1' ++ insn_call rid false ca rt1 va1 fv lp :: cs) tmn))
-  (Hinscope : wf_ExecutionContext pinfo stinfo (los,nts) Mem gl
-               {|
-               Opsem.CurFunction := F;
-               Opsem.CurBB := (l1, stmts_intro ps1
-                                (cs1' ++
-                                 insn_call rid noret0 ca rt1 va1 fv lp :: cs) tmn);
-               Opsem.CurCmds := insn_call rid noret0 ca rt1 va1 fv lp :: cs;
-               Opsem.Terminator := tmn;
-               Opsem.Locals := lc;
-               Opsem.Allocas := als |}),
-   wf_ExecutionContext pinfo stinfo (los,nts) Mem' gl
-     {|
-     Opsem.CurFunction := F;
-     Opsem.CurBB := (l1, stmts_intro ps1
-                      (cs1' ++ insn_call rid noret0 ca rt1 va1 fv lp :: cs) tmn);
-     Opsem.CurCmds := cs;
-     Opsem.Terminator := tmn;
-     Opsem.Locals := lc';
-     Opsem.Allocas := als |}.
-Proof.
-  intros.
-  intros J1 J2 J3. simpl in J1, J2, J3. simpl. subst.
-  assert (J2':=J2).
-  apply follow_alive_store_cons in J2; auto.
-  apply Hinscope in J2; auto.
-  simpl in J2.
-  intros gvsa gvsv Hlka Hlkv.
-  unfold Opsem.exCallUpdateLocals in H5.
-  destruct noret0.
-    inv H5.
-    eapply J2 in Hlkv; eauto.
-    eapply MemProps.callExternalOrIntrinsics_preserves_mload; eauto.
-
-    destruct oresult; inv H5.
-    remember (fit_gv (los,nts) rt1 g) as R.
-    destruct R; inv H0.
-    assert (rid <> PI_id pinfo) as Hneq.
-      eapply WF_PhiInfo_spec10 in HBinF; eauto.
-    rewrite <- lookupAL_updateAddAL_neq in Hlka; auto.
-    assert (used_in_value rid (SI_value pinfo stinfo) = false) as Hnouse.
-      eapply alive_store_doesnt_use_its_followers; eauto
-        using wf_system__wf_fdef, follow_alive_store_cons.
-    apply getOperandValue_updateAddAL_nouse in Hlkv; auto.
-    eapply MemProps.callExternalOrIntrinsics_preserves_mload; eauto.
-Qed.
-
-Ltac destruct_ctx_other :=
-match goal with
-| Hwfcfg : OpsemPP.wf_Config ?cfg,
-  Hwfpp : OpsemPP.wf_State ?cfg _,
-  HwfS1 : wf_State _ _ _ _,
-  Hnoalias : Promotability.wf_State _ _ _ _ |- _ =>
-  destruct Hwfcfg as [_ [Hwfgl0 [HwfSystem HmInS]]];
-  destruct Hwfpp as 
-    [Hnonempty [
-     [Hreach1 [HBinF1 [HFinPs1 [Hwflc1 [_ [l1 [ps1 [cs1' Heq1]]]]]]]]
-     [HwfEC0 HwfCall]
-    ]]; subst;
-  fold (@OpsemPP.wf_ECStack DGVs) in HwfEC0;
-  destruct HwfS1 as [Hinscope HwfECs]; simpl;
-  simpl in Hinscope, HwfECs;
-  fold wf_ECStack in HwfECs;
-  destruct Hnoalias as
-    [
-      [[Hinscope' _] [HwfECs' HwfHT]]
-      [[Hdisjals _] HwfM]
-    ]; simpl in Hdisjals;
-  fold Promotability.wf_ECStack in HwfECs'
-end.
-
-Ltac preservation_malloc :=
-  destruct_ctx_other;
-  split; simpl; try solve [
-    eapply malloc_preserves_wf_EC_at_head;
-      eauto using wf_system__wf_fdef, wf_system__uniqFdef |
-    eapply malloc_preserves_wf_ECStack_in_tail; eauto].
-
-Ltac preservation_pure_cmd_updated_case_helper:=
-  destruct_ctx_other;
-  intros; subst;
-  split; try
-  eapply alive_store_doesnt_use_its_followers; try solve [
-    eauto using wf_system__wf_fdef |
-    match goal with
-    | HBinF1 : blockInFdefB (_, stmts_intro _ (_ ++ _ :: _) _) _ = true |- _ =>
-       eapply WF_PhiInfo_spec10 in HBinF1; eauto using wf_system__uniqFdef
-    end].
-
-Ltac preservation_pure_cmd_updated_case:=
-  abstract (eapply preservation_pure_cmd_updated_case; eauto; try solve
-    [simpl; auto | preservation_pure_cmd_updated_case_helper]).
-
-Ltac free_preserves_wf_EC_at_head :=
-  match goal with
-| Hinscope: wf_ExecutionContext ?pinfo _ _ _ _ _ |- _ =>
-  intros J1 J2 J3; simpl in J1, J2, J3; simpl; subst;
-  assert (J2':=J2);
-  apply follow_alive_store_cons in J2; eauto using wf_system__uniqFdef;
-  apply Hinscope in J2; auto; simpl in J2;
-  destruct (fdef_dec (PI_f pinfo) (PI_f pinfo)); try congruence;
-  intros gvsa gvsv Hlkpa Hlkpv;
-  eapply J2 in Hlkpv; eauto;
-  eapply free_preserves_mload; try solve [
-    eauto |
-    eapply operand__no_alias_with__head; try solve [
-      eauto | preservation_tac2 | get_wf_value_for_simop; eauto]
-    ]
-end.
-
 Lemma preservation : forall maxb pinfo stinfo cfg S1 S2 tr
   (Hwfg: wf_globals maxb (OpsemAux.Globals cfg))
   (Hwfcfg: OpsemPP.wf_Config cfg) (Hwfpp: OpsemPP.wf_State cfg S1) 
@@ -1010,72 +196,10 @@ Lemma preservation : forall maxb pinfo stinfo cfg S1 S2 tr
   (HwfS1: wf_State pinfo stinfo cfg S1), wf_State pinfo stinfo cfg S2.
 Proof.
   intros.
-  (sInsn_cases (induction HsInsn) Case); destruct TD as [los nts]; simpl HwfS1.
-
-Case "sReturn". abstract (eapply preservation_return; eauto).
-Case "sReturnVoid". abstract (eapply preservation_return_void; eauto).
-Case "sBranch". abstract preservation_sBranch.
-Case "sBranch_uncond". abstract preservation_sBranch.
-
-Case "sBop". preservation_pure_cmd_updated_case.
-Case "sFBop". preservation_pure_cmd_updated_case.
-Case "sExtractValue". preservation_pure_cmd_updated_case.
-Case "sInsertValue". preservation_pure_cmd_updated_case.
-
-Case "sMalloc". abstract preservation_malloc.
-
-Case "sFree".
-  abstract
-  (destruct_ctx_other;
-   split; simpl; try solve [
-    free_preserves_wf_EC_at_head |
-    eapply free_preserves_wf_ECStack_in_tail; try solve [
-      eauto | get_wf_value_for_simop; eauto]
-   ]).
-
-Case "sAlloca". abstract preservation_malloc.
-
-Case "sLoad". preservation_pure_cmd_updated_case.
-
-Case "sStore".
-   abstract
-   (destruct_ctx_other;
-    split; simpl; try solve [
-     eapply mstore_preserves_wf_EC_at_head; try solve [
-       eauto using wf_system__uniqFdef |
-       get_wf_value_for_simop; eauto
-     ] |
-     match goal with
-     | _ : ?gv1 @ ?gvs1', _ : ?mp2 @ ?mps2',
-       _ : mstore _ _ ?mp2 _ ?gv1 _ = _ |- _ =>
-       eapply mstore_preserves_wf_ECStack_in_tail
-         with (gvs1:=gvs1')(mps2:=mps2'); 
-         try solve [eauto | get_wf_value_for_simop; eauto]
-     end]).
-
-Case "sGEP". preservation_pure_cmd_updated_case.
-Case "sTrunc". preservation_pure_cmd_updated_case.
-Case "sExt". preservation_pure_cmd_updated_case.
-Case "sCast". preservation_pure_cmd_updated_case.
-Case "sIcmp". preservation_pure_cmd_updated_case.
-Case "sFcmp". preservation_pure_cmd_updated_case.
-Case "sSelect". destruct (isGVZero (los, nts) c); preservation_pure_cmd_updated_case.
-
-Case "sCall".
-  abstract (
-  destruct_ctx_other;
-  split; try solve [
-    intros J1 J2 J3; simpl in J1, J2, J3; simpl;
-    eapply follow_alive_store_at_beginning_false in J2; eauto; inv J2 |
-    split; auto]).
-
-Case "sExCall".
-  abstract (
-  destruct_ctx_other;
-  split; simpl; try solve [
-    eapply callExternalFunction_preserves_wf_ECStack_at_head; eauto using
-      wf_system__wf_fdef, wf_system__uniqFdef |
-    eapply callExternalFunction_preserves_wf_ECStack_in_tail; eauto]).
+  destruct (stinfo__minfo pinfo stinfo) as [minfo Heq].
+  eapply stinfo__wf_State__minfo; eauto.
+  eapply stinfo__wf_State__minfo in HwfS1; eauto.
+  eapply alive_mop.preservation; eauto.
 Qed.
 
 Lemma preservation_star : forall maxb pinfo stinfo cfg S1 S2 tr
@@ -1113,19 +237,7 @@ Lemma s_genInitState__alive_store: forall S main VarArgs cfg IS pinfo stinfo
   wf_State pinfo stinfo cfg IS.
 Proof.
   intros.
-  simpl_s_genInitState. 
-  split; simpl; auto.
-  unfold wf_ExecutionContext. simpl.
-  intros.
-  unfold wf_defs.
-  intros.
-  apply getParentOfFdefFromSystem__moduleInProductsInSystemB in HeqR0.
-  destruct HeqR0 as [J1 J2].
-  rewrite H in *.
-  eapply wf_system__uniqFdef in J1; eauto.
-  replace a with (getArgsOfFdef (PI_f pinfo)) in HeqR3.
-    erewrite WF_PhiInfo__pid_isnt_in_init in Hlkpa; eauto.
-    congruence.
-
-    rewrite <- H. auto.
+  destruct (stinfo__minfo pinfo stinfo) as [minfo Heq].
+  eapply stinfo__wf_State__minfo; eauto.
+  eapply alive_mop.s_genInitState__alive_mop; eauto.
 Qed.
